capDL+drefine: restyle capDL spec
Restyle capDL spec according to current style guide; minimal DRefine
update.

- definition/function style
- indentation
- parentheses
- comment style
- minor adjustments to comment contents
- some (rare) changes might affect proofs:
  - changes to some bound names
  - removal/addition of $
  - change of = into ==
- no other content changes, in particular no change of if/case into
  when/maybeM or other monad idioms

Signed-off-by: Gerwin Klein <gerwin.klein@proofcraft.systems>

spec/capDL/CSpace_D.thy
@@ -4,245 +4,203 @@
  * SPDX-License-Identifier: GPL-2.0-only
  *)
 
-(*
- * Operations on CSpace
- *)
+(* Operations on CSpace *)
 
 theory CSpace_D
-imports
-  PageTableUnmap_D
+  imports
+    PageTableUnmap_D
 begin
 
 (* Does the given cap have any children? *)
-definition
-  has_children :: "cdl_cap_ref \<Rightarrow> cdl_state \<Rightarrow> bool"
-where
+definition has_children :: "cdl_cap_ref \<Rightarrow> cdl_state \<Rightarrow> bool" where
   "has_children parent s = (\<exists>child. is_cdt_parent s parent child)"
 
-(*
- * Ensure that the given cap does not contain any children
- * in the CDT.
- *)
-definition
-  ensure_no_children :: "cdl_cap_ref \<Rightarrow> unit except_monad"
-where
+definition ensure_no_children :: "cdl_cap_ref \<Rightarrow> unit except_monad" where
   "ensure_no_children x \<equiv> doE
      c \<leftarrow> liftE $ gets (has_children x);
      whenE c $ throw
    odE"
 
 (* Ensure that the given cap slot is empty. *)
-definition
-  ensure_empty :: "cdl_cap_ref \<Rightarrow> unit except_monad"
-where
+definition ensure_empty :: "cdl_cap_ref \<Rightarrow> unit except_monad" where
   "ensure_empty cap_ref \<equiv> doE
      cap \<leftarrow> liftE $ get_cap cap_ref;
      unlessE (cap = NullCap) $ throw
-  odE"
+   odE"
 
 (* Insert a new cap into an object. The cap will have no parent. *)
-definition
-  insert_cap_orphan :: "cdl_cap \<Rightarrow> cdl_cap_ref \<Rightarrow> unit k_monad"
-where
+definition insert_cap_orphan :: "cdl_cap \<Rightarrow> cdl_cap_ref \<Rightarrow> unit k_monad" where
   "insert_cap_orphan new_cap dest_slot \<equiv> do
      old_cap \<leftarrow> get_cap dest_slot;
      assert (old_cap = NullCap);
      set_cap dest_slot new_cap
    od"
 
-primrec (nonexhaustive)
-  untyped_cap_range :: "cdl_cap \<Rightarrow> cdl_object_id set"
-where
+primrec (nonexhaustive) untyped_cap_range :: "cdl_cap \<Rightarrow> cdl_object_id set" where
   "untyped_cap_range (UntypedCap _ r available) = r"
 
-primrec (nonexhaustive)
-  available_range :: "cdl_cap \<Rightarrow> cdl_object_id set"
-where
+primrec (nonexhaustive) available_range :: "cdl_cap \<Rightarrow> cdl_object_id set" where
   "available_range (UntypedCap _ r available) = available"
 
-definition
-  set_available_range :: "cdl_cap \<Rightarrow> cdl_object_id set \<Rightarrow> cdl_cap"
-where
+definition set_available_range :: "cdl_cap \<Rightarrow> cdl_object_id set \<Rightarrow> cdl_cap" where
   "set_available_range cap nrange \<equiv>
-    case cap of UntypedCap d r available \<Rightarrow> UntypedCap d r nrange | _ \<Rightarrow> cap"
+     case cap of UntypedCap d r available \<Rightarrow> UntypedCap d r nrange | _ \<Rightarrow> cap"
 
 lemmas set_avaiable_range_simps[simp] = set_available_range_def[split_simps cdl_cap.split]
 
-definition
-  set_untyped_cap_as_full :: "cdl_cap \<Rightarrow> cdl_cap \<Rightarrow> cdl_cap_ref \<Rightarrow> unit k_monad"
-where
+definition set_untyped_cap_as_full :: "cdl_cap \<Rightarrow> cdl_cap \<Rightarrow> cdl_cap_ref \<Rightarrow> unit k_monad" where
   "set_untyped_cap_as_full src_cap new_cap src_slot \<equiv>
-  if (is_untyped_cap src_cap \<and> is_untyped_cap new_cap
-     \<and> cap_objects src_cap = cap_objects new_cap) then
-     (set_cap src_slot (set_available_range src_cap {}))
+     if is_untyped_cap src_cap \<and> is_untyped_cap new_cap \<and> cap_objects src_cap = cap_objects new_cap
+     then set_cap src_slot (set_available_range src_cap {})
      else return ()"
 
 (* Insert a new cap into an object. The cap will be a sibling. *)
-definition
-  insert_cap_sibling :: "cdl_cap \<Rightarrow> cdl_cap_ref \<Rightarrow> cdl_cap_ref \<Rightarrow> unit k_monad"
-where
+definition insert_cap_sibling :: "cdl_cap \<Rightarrow> cdl_cap_ref \<Rightarrow> cdl_cap_ref \<Rightarrow> unit k_monad" where
   "insert_cap_sibling new_cap src_slot dest_slot \<equiv> do
-    src_cap \<leftarrow> get_cap src_slot;
-    old_cap \<leftarrow> get_cap dest_slot;
-    assert (old_cap = NullCap);
-    set_untyped_cap_as_full src_cap new_cap src_slot;
-    set_cap dest_slot new_cap;
-    p \<leftarrow> gets $ opt_parent src_slot;
-    case p of
-      None \<Rightarrow> return ()
-    | Some parent \<Rightarrow> set_parent dest_slot parent
-  od"
+     src_cap \<leftarrow> get_cap src_slot;
+     old_cap \<leftarrow> get_cap dest_slot;
+     assert (old_cap = NullCap);
+     set_untyped_cap_as_full src_cap new_cap src_slot;
+     set_cap dest_slot new_cap;
+     p \<leftarrow> gets $ opt_parent src_slot;
+     case p of
+       None \<Rightarrow> return ()
+     | Some parent \<Rightarrow> set_parent dest_slot parent
+   od"
 
 (* Insert a new cap into an object. The cap will be a child. *)
-definition
-  insert_cap_child :: "cdl_cap \<Rightarrow> cdl_cap_ref \<Rightarrow> cdl_cap_ref \<Rightarrow> unit k_monad"
-where
+definition insert_cap_child :: "cdl_cap \<Rightarrow> cdl_cap_ref \<Rightarrow> cdl_cap_ref \<Rightarrow> unit k_monad" where
   "insert_cap_child new_cap src_slot dest_slot \<equiv> do
-    src_cap \<leftarrow> get_cap src_slot;
-    old_cap \<leftarrow> get_cap dest_slot;
-    assert (old_cap = NullCap);
-    set_untyped_cap_as_full src_cap new_cap src_slot;
-    set_cap dest_slot new_cap;
-    set_parent dest_slot src_slot
-  od"
+     src_cap \<leftarrow> get_cap src_slot;
+     old_cap \<leftarrow> get_cap dest_slot;
+     assert (old_cap = NullCap);
+     set_untyped_cap_as_full src_cap new_cap src_slot;
+     set_cap dest_slot new_cap;
+     set_parent dest_slot src_slot
+   od"
 
-(*
- * Delete an ASID pool.
- *)
-definition
-  delete_asid_pool :: "cdl_cnode_index \<Rightarrow> cdl_object_id \<Rightarrow> unit k_monad"
-where
+(* Delete an ASID pool. *)
+definition delete_asid_pool :: "cdl_cnode_index \<Rightarrow> cdl_object_id \<Rightarrow> unit k_monad" where
   "delete_asid_pool base ptr \<equiv> do
-    asid_table \<leftarrow> gets cdl_asid_table;
-    asid_table' \<leftarrow> return $ asid_table (base \<mapsto> NullCap);
-    modify (\<lambda>s. s \<lparr>cdl_asid_table := asid_table'\<rparr>)
-  od \<sqinter> return ()"
+     asid_table \<leftarrow> gets cdl_asid_table;
+     asid_table' \<leftarrow> return $ asid_table (base \<mapsto> NullCap);
+     modify (\<lambda>s. s \<lparr>cdl_asid_table := asid_table'\<rparr>)
+   od \<sqinter> return ()"
 
-(*
- * Delete a particular ASID, decactivating the PD using it
- * in the process.
- *)
-definition
-  delete_asid :: "cdl_asid \<Rightarrow> cdl_object_id \<Rightarrow> unit k_monad"
-where
+(* Delete a particular ASID, decactivating the PD using it  in the process. *)
+definition delete_asid :: "cdl_asid \<Rightarrow> cdl_object_id \<Rightarrow> unit k_monad" where
   "delete_asid asid pd \<equiv> do
-    asid_table \<leftarrow> gets cdl_asid_table;
-    case asid_table (fst asid) of
+     asid_table \<leftarrow> gets cdl_asid_table;
+     case asid_table (fst asid) of
        Some NullCap \<Rightarrow> return ()
      | Some (AsidPoolCap p _) \<Rightarrow> set_cap (p, (snd asid)) NullCap
      | _ \<Rightarrow> fail
-  od \<sqinter> return ()"
+   od \<sqinter> return ()"
 
-definition
-  get_irq_slot :: "cdl_irq \<Rightarrow> cdl_state \<Rightarrow> cdl_cap_ref"
-where
+definition get_irq_slot :: "cdl_irq \<Rightarrow> cdl_state \<Rightarrow> cdl_cap_ref" where
   "get_irq_slot irq s \<equiv> (cdl_irq_node s irq, 0)"
 
 text \<open>Actions to be taken after deleting an IRQ Handler capability.\<close>
-definition
-  deleting_irq_handler :: "cdl_irq \<Rightarrow> unit k_monad"
-where
- "deleting_irq_handler irq \<equiv>
-    gets (get_irq_slot irq) >>= delete_cap_simple"
+definition deleting_irq_handler :: "cdl_irq \<Rightarrow> unit k_monad" where
+  "deleting_irq_handler irq \<equiv> gets (get_irq_slot irq) >>= delete_cap_simple"
 
-definition
-  cancel_ipc ::"cdl_object_id \<Rightarrow> unit k_monad"
-  where "cancel_ipc ptr \<equiv>
-  do cap \<leftarrow> KHeap_D.get_cap (ptr,tcb_pending_op_slot);
-   (case cap of
-    PendingSyncRecvCap _ is_reply _ \<Rightarrow> ( do
-     when is_reply $ update_thread_fault ptr (\<lambda>x. False);
-     revoke_cap_simple (ptr,tcb_replycap_slot);
-     when (\<not> is_reply) $ set_cap (ptr,tcb_pending_op_slot) NullCap
-     od )
-   | PendingSyncSendCap _ _ _ _ _ _ \<Rightarrow> (do
-     revoke_cap_simple (ptr,tcb_replycap_slot);
-     set_cap (ptr,tcb_pending_op_slot) NullCap
-     od)
-   | PendingNtfnRecvCap _ \<Rightarrow> (do
-     revoke_cap_simple (ptr,tcb_replycap_slot);
-     set_cap (ptr, tcb_pending_op_slot) NullCap
-     od)
-   | _ \<Rightarrow> return ())
-  od"
+definition cancel_ipc ::"cdl_object_id \<Rightarrow> unit k_monad" where
+  "cancel_ipc ptr \<equiv> do
+     cap \<leftarrow> get_cap (ptr, tcb_pending_op_slot);
+     case cap of
+       PendingSyncRecvCap _ is_reply _ \<Rightarrow> do
+         when is_reply $ update_thread_fault ptr (\<lambda>x. False);
+         revoke_cap_simple (ptr,tcb_replycap_slot);
+         when (\<not> is_reply) $ set_cap (ptr,tcb_pending_op_slot) NullCap
+       od
+     | PendingSyncSendCap _ _ _ _ _ _ \<Rightarrow> do
+         revoke_cap_simple (ptr,tcb_replycap_slot);
+         set_cap (ptr,tcb_pending_op_slot) NullCap
+       od
+     | PendingNtfnRecvCap _ \<Rightarrow> do
+         revoke_cap_simple (ptr,tcb_replycap_slot);
+         set_cap (ptr, tcb_pending_op_slot) NullCap
+       od
+     | _ \<Rightarrow> return ()
+   od"
 
-definition
-  prepare_thread_delete ::"cdl_object_id \<Rightarrow> unit k_monad"
-  where "prepare_thread_delete ptr \<equiv> return ()" (* for ARM it does nothing *)
+definition prepare_thread_delete ::"cdl_object_id \<Rightarrow> unit k_monad" where
+  "prepare_thread_delete ptr \<equiv> return ()" (* for ARM it does nothing *)
 
-text \<open>Actions that must be taken when a capability is deleted. Returns a
-Zombie capability if deletion requires a long-running operation and also a
-possible IRQ to be cleared.\<close>
-fun
-  finalise_cap :: "cdl_cap \<Rightarrow> bool \<Rightarrow> (cdl_cap \<times> cdl_cap) k_monad"
-where
-  "finalise_cap NullCap                  final = return (NullCap, NullCap)"
-| "finalise_cap RestartCap               final = return (NullCap, NullCap)"
-| "finalise_cap (UntypedCap dev r a)           final = return (NullCap, NullCap)"
-| "finalise_cap (EndpointCap r b R)      final =
-      (liftM (K (NullCap, NullCap)) $ when  final $ cancel_all_ipc r)"
-| "finalise_cap (NotificationCap r b R) final =
-      (liftM (K (NullCap, NullCap)) $ when  final $
-       do
-         unbind_maybe_notification r;
-         cancel_all_ipc r
-       od)"
-| "finalise_cap (ReplyCap r R)           final = return (NullCap, NullCap)"
-| "finalise_cap (MasterReplyCap r)       final = return (NullCap, NullCap)"
-| "finalise_cap (CNodeCap r bits g sz)   final =
-      (return (if final then ZombieCap r else NullCap, NullCap))"
-| "finalise_cap (TcbCap r)               final =
-      (do
-         when final $ (do unbind_notification r;
+text \<open>
+  Actions that must be taken when a capability is deleted. Returns a
+  Zombie capability if deletion requires a long-running operation and also a
+  possible IRQ to be cleared.\<close>
+fun finalise_cap :: "cdl_cap \<Rightarrow> bool \<Rightarrow> (cdl_cap \<times> cdl_cap) k_monad" where
+    "finalise_cap NullCap final = return (NullCap, NullCap)"
+  | "finalise_cap RestartCap final = return (NullCap, NullCap)"
+  | "finalise_cap (UntypedCap dev r a) final = return (NullCap, NullCap)"
+  | "finalise_cap (EndpointCap r b R) final =
+       liftM (K (NullCap, NullCap)) (when final $ cancel_all_ipc r)"
+  | "finalise_cap (NotificationCap r b R) final =
+       liftM (K (NullCap, NullCap))
+             (when final $ do
+                unbind_maybe_notification r;
+                cancel_all_ipc r
+              od)"
+  | "finalise_cap (ReplyCap r R) final = return (NullCap, NullCap)"
+  | "finalise_cap (MasterReplyCap r) final = return (NullCap, NullCap)"
+  | "finalise_cap (CNodeCap r bits g sz) final =
+       return (if final then ZombieCap r else NullCap, NullCap)"
+  | "finalise_cap (TcbCap r) final = do
+       when final $ do
+         unbind_notification r;
          cancel_ipc r;
-         KHeap_D.set_cap (r, tcb_pending_op_slot) cdl_cap.NullCap;
-         prepare_thread_delete r od);
-         return (if final then (ZombieCap r) else NullCap, NullCap)
-       od)"
-| "finalise_cap (PendingSyncSendCap r _ _ _ _ _) final = return (NullCap, NullCap)"
-| "finalise_cap (PendingSyncRecvCap r _ _) final = return (NullCap, NullCap)"
-| "finalise_cap (PendingNtfnRecvCap r)  final = return (NullCap, NullCap)"
-| "finalise_cap IrqControlCap            final = return (NullCap, NullCap)"
-| "finalise_cap (IrqHandlerCap irq)      final = (
+         set_cap (r, tcb_pending_op_slot) cdl_cap.NullCap;
+         prepare_thread_delete r
+       od;
+       return (if final then ZombieCap r else NullCap, NullCap)
+     od"
+  | "finalise_cap (PendingSyncSendCap r _ _ _ _ _) final = return (NullCap, NullCap)"
+  | "finalise_cap (PendingSyncRecvCap r _ _) final = return (NullCap, NullCap)"
+  | "finalise_cap (PendingNtfnRecvCap r) final = return (NullCap, NullCap)"
+  | "finalise_cap IrqControlCap final = return (NullCap, NullCap)"
+  | "finalise_cap (IrqHandlerCap irq) final = (
        if final then do
          deleting_irq_handler irq;
          return (NullCap, (IrqHandlerCap irq))
        od
        else return (NullCap, NullCap))"
-| "finalise_cap (ZombieCap r)            final =
-      (do assert final; return (ZombieCap r, NullCap) od)"
-| "finalise_cap (AsidPoolCap ptr asid)        final = (
+  | "finalise_cap (ZombieCap r) final = do
+       assert final; return (ZombieCap r, NullCap)
+     od"
+  | "finalise_cap (AsidPoolCap ptr asid)        final = (
        if final then do
          delete_asid_pool asid ptr;
          return (NullCap, NullCap)
        od
        else return (NullCap, NullCap))"
-| "finalise_cap AsidControlCap           final = return (NullCap,NullCap)"
-| "finalise_cap (PageTableCap PD ptr x (Some (asid, _))) final = (
+  | "finalise_cap AsidControlCap final = return (NullCap,NullCap)"
+  | "finalise_cap (PageTableCap PD ptr x (Some (asid, _))) final = (
        if final \<and> x = Real then do
          delete_asid asid ptr;
          return (NullCap, NullCap)
        od
        else return (NullCap, NullCap))"
-| "finalise_cap (PageTableCap PT ptr x (Some asid)) final = (
-       if (final \<and> x = Real) then do
+  | "finalise_cap (PageTableCap PT ptr x (Some asid)) final = (
+       if final \<and> x = Real then do
          unmap_page_table asid ptr;
          return (NullCap, NullCap)
        od
        else return (NullCap, NullCap))"
-| "finalise_cap (FrameCap dev ptr _ s x (Some asid)) final = (
+  | "finalise_cap (FrameCap dev ptr _ s x (Some asid)) final = (
        if x = Real then do
          unmap_page asid ptr s;
          return (NullCap, NullCap)
        od
        else return (NullCap, NullCap))"
-| "finalise_cap _ final = return (NullCap, NullCap)"
+  | "finalise_cap _ final = return (NullCap, NullCap)"
 
 
-text \<open>The fast_finalise operation is used to delete a capability when it is
-known that a long-running operation is impossible. It is equivalent to calling
-the regular finalise operation. It cannot be defined in that way as doing so
-would create a circular definition.\<close>
+text \<open>
+  The fast_finalise operation is used to delete a capability when it is known that a long-running
+  operation is impossible. It is equivalent to calling the regular finalise operation. It cannot be
+  defined in that way as doing so would create a circular definition.\<close>
 lemma fast_finalise_def2:
   "fast_finalise cap final = do
      assert (can_fast_finalise cap);
@@ -252,235 +210,175 @@ lemma fast_finalise_def2:
   unfolding can_fast_finalise_def
   by (rule finalise_cap.cases[of "(cap,final)"]; simp add: assert_def liftM_def)
 
-(*
- * Atomically swap the two given caps.
- *)
-
-definition
-  swap_cap :: "cdl_cap \<Rightarrow> cdl_cap_ref \<Rightarrow> cdl_cap \<Rightarrow> cdl_cap_ref \<Rightarrow> unit k_monad"
-where
+(* Atomically swap the two given caps. *)
+definition swap_cap :: "cdl_cap \<Rightarrow> cdl_cap_ref \<Rightarrow> cdl_cap \<Rightarrow> cdl_cap_ref \<Rightarrow> unit k_monad" where
   "swap_cap cap1 slot1 cap2 slot2 \<equiv> do
      set_cap slot1 cap2;
      set_cap slot2 cap1;
      swap_parents slot1 slot2
-  od"
+   od"
 
-(*
- * Move the given cap from one location to another,
- * possibly modifying it along the way.
- *)
-definition
-  move_cap :: "cdl_cap \<Rightarrow> cdl_cap_ref \<Rightarrow> cdl_cap_ref \<Rightarrow> unit k_monad"
-where
+(* Move the given cap from one location to another, possibly modifying it along the way. *)
+definition move_cap :: "cdl_cap \<Rightarrow> cdl_cap_ref \<Rightarrow> cdl_cap_ref \<Rightarrow> unit k_monad" where
   "move_cap cap src_slot dest_slot \<equiv> do
      insert_cap_orphan cap dest_slot;
      set_cap src_slot NullCap;
      swap_parents src_slot dest_slot
-  od"
+   od"
 
-definition
-  monadic_rel_optionation_form :: "('a \<Rightarrow> ('s, 'b) nondet_monad)
-      \<Rightarrow> (('a \<times> 's) option \<times> ('b \<times> 's) option) set"
-where
- "monadic_rel_optionation_form f =
-    {(x, y). (x \<noteq> None \<and> y \<noteq> None \<and> the y \<in> fst (case_prod f (the x)))
-           \<or> (x \<noteq> None \<and> y = None \<and> snd (case_prod f (the x)))
-           \<or> (x = None \<and> y = None)}"
+definition monadic_rel_optionation_form ::
+  "('a \<Rightarrow> ('s, 'b) nondet_monad) \<Rightarrow> (('a \<times> 's) option \<times> ('b \<times> 's) option) set"
+  where
+  "monadic_rel_optionation_form f =
+     {(x, y). (x \<noteq> None \<and> y \<noteq> None \<and> the y \<in> fst (case_prod f (the x))) \<or>
+              (x \<noteq> None \<and> y = None \<and> snd (case_prod f (the x))) \<or>
+              (x = None \<and> y = None)}"
 
-definition
-  monadic_option_dest :: "('a \<times> 's) option set \<Rightarrow> (('a \<times> 's) set \<times> bool)"
-where
- "monadic_option_dest S = (Some -` S, None \<in> S)"
+definition monadic_option_dest :: "('a \<times> 's) option set \<Rightarrow> (('a \<times> 's) set \<times> bool)" where
+  "monadic_option_dest S = (Some -` S, None \<in> S)"
 
 lemma use_option_form:
   "f x = (\<lambda>s. monadic_option_dest  (monadic_rel_optionation_form f `` {Some (x, s)}))"
   by (simp add: monadic_rel_optionation_form_def monadic_option_dest_def)
 
-lemma ex_option: " (\<exists>x. P x) = ((\<exists>y. P (Some y)) \<or> P None)"
-  apply safe
-  apply (case_tac x, auto)
-  done
+lemma ex_option:
+  "(\<exists>x. P x) = ((\<exists>y. P (Some y)) \<or> P None)"
+  by (metis not_None_eq)
 
 lemma use_option_form_bind:
-  "f x >>= g = (\<lambda>s. monadic_option_dest
-       ((monadic_rel_optionation_form f O monadic_rel_optionation_form g) `` {Some (x, s)}))"
-  apply (rule ext)
-  apply (simp add: monadic_rel_optionation_form_def monadic_option_dest_def
-                   bind_def split_def)
-  apply (simp add: relcomp_unfold ex_option image_def prod_eq_iff Bex_def)
-  apply fastforce
-  done
+  "f x >>= g =
+   (\<lambda>s. monadic_option_dest
+         ((monadic_rel_optionation_form f O monadic_rel_optionation_form g) `` {Some (x, s)}))"
+  by (fastforce simp: monadic_rel_optionation_form_def monadic_option_dest_def bind_def
+                      relcomp_unfold ex_option image_def prod_eq_iff Bex_def)
 
-definition
-  monadic_trancl :: "('a \<Rightarrow> ('s, 'a) nondet_monad)
-       \<Rightarrow> 'a \<Rightarrow> ('s, 'a) nondet_monad"
-where
- "monadic_trancl f x = (\<lambda>s. monadic_option_dest ((monadic_rel_optionation_form f)\<^sup>* `` {Some (x, s)}))"
+definition monadic_trancl :: "('a \<Rightarrow> ('s, 'a) nondet_monad) \<Rightarrow> 'a \<Rightarrow> ('s, 'a) nondet_monad" where
+  "monadic_trancl f x =
+     (\<lambda>s. monadic_option_dest ((monadic_rel_optionation_form f)\<^sup>* `` {Some (x, s)}))"
 
-definition
-  monadic_trancl_preemptible ::
-     "('a \<Rightarrow> ('s, 'e + 'a) nondet_monad)
-         \<Rightarrow> ('a \<Rightarrow> ('s, 'e + 'a) nondet_monad)"
-where
- "monadic_trancl_preemptible f x
-    = monadic_trancl (lift f) (Inr x)"
+definition monadic_trancl_preemptible ::
+  "('a \<Rightarrow> ('s, 'e + 'a) nondet_monad) \<Rightarrow> ('a \<Rightarrow> ('s, 'e + 'a) nondet_monad)"
+  where
+  "monadic_trancl_preemptible f x = monadic_trancl (lift f) (Inr x)"
 
-definition
-  cap_removeable :: "cdl_cap \<Rightarrow> cdl_cap_ref \<Rightarrow> cdl_state \<Rightarrow> bool"
-where
- "cap_removeable cap slot s =
-   (cap = NullCap
-      \<or> (\<exists>p. cap = ZombieCap p \<and> swp opt_cap s ` (({p} \<times> UNIV) - {slot})
-              \<subseteq> {Some NullCap, None}))"
+definition cap_removeable :: "cdl_cap \<Rightarrow> cdl_cap_ref \<Rightarrow> cdl_state \<Rightarrow> bool" where
+  "cap_removeable cap slot s \<equiv>
+     cap = NullCap \<or>
+     (\<exists>p. cap = ZombieCap p \<and> swp opt_cap s ` (({p} \<times> UNIV) - {slot}) \<subseteq> {Some NullCap, None})"
 
-definition
-  finalise_slot_inner1 :: "cdl_cap_ref \<Rightarrow> (cdl_cap \<times> bool) k_monad"
-where
- "finalise_slot_inner1 victim = do
-    cap \<leftarrow> get_cap victim;
-    final \<leftarrow> is_final_cap cap;
-    (cap', irqopt) \<leftarrow> finalise_cap cap final;
-    removeable \<leftarrow> gets $ cap_removeable cap' victim;
-    when (\<not> removeable) (set_cap victim cap')
-        \<sqinter> set_cap victim cap';
-    return (cap', removeable)
-  od"
+definition finalise_slot_inner1 :: "cdl_cap_ref \<Rightarrow> (cdl_cap \<times> bool) k_monad" where
+  "finalise_slot_inner1 victim = do
+     cap \<leftarrow> get_cap victim;
+     final \<leftarrow> is_final_cap cap;
+     (cap', irqopt) \<leftarrow> finalise_cap cap final;
+     removeable \<leftarrow> gets $ cap_removeable cap' victim;
+     when (\<not>removeable) (set_cap victim cap') \<sqinter> set_cap victim cap';
+     return (cap', removeable)
+   od"
 
-definition
-  get_zombie_range :: "cdl_cap \<Rightarrow> cdl_state \<Rightarrow> cdl_cap_ref set"
-where
- "get_zombie_range cap =
-    (\<lambda>s. case cap of ZombieCap p \<Rightarrow> dom (swp opt_cap s) \<inter> ({p} \<times> UNIV)
-               | _ \<Rightarrow> {})"
+definition get_zombie_range :: "cdl_cap \<Rightarrow> cdl_state \<Rightarrow> cdl_cap_ref set" where
+  "get_zombie_range cap \<equiv>
+    \<lambda>s. case cap of ZombieCap p \<Rightarrow> dom (swp opt_cap s) \<inter> ({p} \<times> UNIV) | _ \<Rightarrow> {}"
 
-definition
-  swap_for_delete :: "cdl_cap_ref \<Rightarrow> cdl_cap_ref \<Rightarrow> unit k_monad"
-where
- "swap_for_delete ptr1 ptr2 = do
-    cap1 \<leftarrow> get_cap ptr1;
-    cap2 \<leftarrow> get_cap ptr2;
-    swap_cap cap1 ptr1 cap2 ptr2
-  od"
+definition swap_for_delete :: "cdl_cap_ref \<Rightarrow> cdl_cap_ref \<Rightarrow> unit k_monad" where
+  "swap_for_delete ptr1 ptr2 = do
+     cap1 \<leftarrow> get_cap ptr1;
+     cap2 \<leftarrow> get_cap ptr2;
+     swap_cap cap1 ptr1 cap2 ptr2
+   od"
 
-definition
- "finalise_slot_inner2 =
-      (\<lambda>(region, finalised).
-        liftE (do (victim', remove) \<leftarrow> select region;
-          (cap', removeable) \<leftarrow> finalise_slot_inner1 victim';
-          region' \<leftarrow> gets $ get_zombie_range cap';
-          return (region \<union> (region' \<times> {True}), if removeable then {(victim', remove)} else {})
-        od) \<sqinter>
-        liftE (do (slot, slot') \<leftarrow> select {(x, y). (x, True) \<in> region \<and> (y, True) \<in> region \<and> x \<noteq> y};
-          swap_for_delete slot slot';
-          return (region, {})
-        od) \<sqinter>
-        liftE (do victim' \<leftarrow> select {x. (x, True) \<in> finalised};
-          empty_slot victim';
-          return (region, {})
-        od) \<sqinter>
-        throw
-      )"
+definition finalise_slot_inner2 where
+  "finalise_slot_inner2 \<equiv>
+     \<lambda>(region, finalised).
+       liftE (do
+         (victim', remove) \<leftarrow> select region;
+         (cap', removeable) \<leftarrow> finalise_slot_inner1 victim';
+         region' \<leftarrow> gets $ get_zombie_range cap';
+         return (region \<union> (region' \<times> {True}), if removeable then {(victim', remove)} else {})
+       od) \<sqinter>
+       liftE (do
+         (slot, slot') \<leftarrow> select {(x, y). (x, True) \<in> region \<and> (y, True) \<in> region \<and> x \<noteq> y};
+         swap_for_delete slot slot';
+         return (region, {})
+       od) \<sqinter>
+       liftE (do
+         victim' \<leftarrow> select {x. (x, True) \<in> finalised};
+         empty_slot victim';
+         return (region, {})
+       od) \<sqinter>
+       throw"
 
-definition
-  finalise_slot :: "cdl_cap_ref \<Rightarrow> unit preempt_monad"
-where
- "finalise_slot victim = doE
-    (region, finalised) \<leftarrow>
-      monadic_trancl_preemptible finalise_slot_inner2
-        ({(victim, False)}, {});
+definition finalise_slot :: "cdl_cap_ref \<Rightarrow> unit preempt_monad" where
+  "finalise_slot victim = doE
+    (region, finalised) \<leftarrow> monadic_trancl_preemptible finalise_slot_inner2 ({(victim, False)}, {});
     whenE (victim \<notin> fst ` finalised) throw
   odE"
 
-definition
-  delete_cap :: "cdl_cap_ref \<Rightarrow> unit preempt_monad"
-where
- "delete_cap victim = doE
-    finalise_slot victim;
-    liftE $ empty_slot victim
-  odE"
+definition delete_cap :: "cdl_cap_ref \<Rightarrow> unit preempt_monad" where
+  "delete_cap victim = doE
+     finalise_slot victim;
+     liftE $ empty_slot victim
+   odE"
 
 
-(*
- * Revoke all the descendants of the given cap.
- *
- * If the CDT is being modelled, this will delete all the
- * descendants of the given cap. Wonderful things happen
- * if we happen to, in this process, delete something
- * that contains the cap we are trying to revoke.
- *)
-definition
-  revoke_cap :: "cdl_cap_ref \<Rightarrow> unit preempt_monad"
-where
+(* Revoke all the descendants of the given cap.
+
+   If the CDT is being modelled, this will delete all the descendants of the given cap. Wonderful
+   things happen if we happen to, in this process, delete something that contains the cap we are
+   trying to revoke. *)
+definition revoke_cap :: "cdl_cap_ref \<Rightarrow> unit preempt_monad" where
   "revoke_cap victim = doE
      fin \<leftarrow> monadic_trancl_preemptible (K (doE
-          S \<leftarrow> liftE $ gets $ descendants_of victim;
-          if S = {} then returnOk True
-          else doE
-            child \<leftarrow> liftE $ select S;
-            cap \<leftarrow> liftE $ get_cap child;
-            assertE (cap \<noteq> NullCap);
-            delete_cap child;
-            Monads_D.throw \<sqinter> returnOk False
-          odE
-       odE)) False;
+       S \<leftarrow> liftE $ gets $ descendants_of victim;
+       if S = {} then returnOk True
+       else doE
+         child \<leftarrow> liftE $ select S;
+         cap \<leftarrow> liftE $ get_cap child;
+         assertE (cap \<noteq> NullCap);
+         delete_cap child;
+         throw \<sqinter> returnOk False
+       odE
+     odE)) False;
      unlessE fin throw
    odE"
 
-(*
- * Get the badge the given thread object is using to
- * perform its IPC send operation.
- *)
-definition
-  get_tcb_ep_badge :: "cdl_tcb \<Rightarrow> cdl_badge option"
-where
+(* Get the badge the given thread object is using to perform its IPC send operation *)
+definition get_tcb_ep_badge :: "cdl_tcb \<Rightarrow> cdl_badge option" where
   "get_tcb_ep_badge t \<equiv>
-    case (cdl_tcb_caps t tcb_pending_op_slot) of
-      Some (PendingSyncSendCap _ badge _ _ _ _) \<Rightarrow> Some badge
-    | _ \<Rightarrow> None"
+     case cdl_tcb_caps t tcb_pending_op_slot of
+       Some (PendingSyncSendCap _ badge _ _ _ _) \<Rightarrow> Some badge
+     | _ \<Rightarrow> None"
 
-(*
- * Cancel all pending send operations to the given endpoint
- * that are using the given badge.
- *)
-definition
-  cancel_badged_sends :: "cdl_object_id \<Rightarrow> cdl_badge \<Rightarrow> unit k_monad"
-where
+(* Cancel all pending send operations to the given endpoint that are using the given badge. *)
+definition cancel_badged_sends :: "cdl_object_id \<Rightarrow> cdl_badge \<Rightarrow> unit k_monad" where
   "cancel_badged_sends ep badge \<equiv>
-    modify (\<lambda>s. s\<lparr>cdl_objects := map_option
-        (\<lambda>obj. case obj of
-            Tcb t \<Rightarrow>
-              if (is_thread_blocked_on_endpoint t ep
-                  \<and> get_tcb_ep_badge t = Some badge) then
-                    Tcb (remove_pending_operation t cdl_cap.RestartCap)
-              else
-                Tcb t
-          | _ \<Rightarrow> obj) \<circ> (cdl_objects s)\<rparr>)"
+     modify (\<lambda>s. s\<lparr>cdl_objects :=
+                     map_option
+                       (\<lambda>obj. case obj of
+                                Tcb t \<Rightarrow> if is_thread_blocked_on_endpoint t ep \<and>
+                                            get_tcb_ep_badge t = Some badge
+                                         then Tcb (remove_pending_operation t cdl_cap.RestartCap)
+                                         else Tcb t
+                              | _ \<Rightarrow> obj)
+                     \<circ> (cdl_objects s)\<rparr>)"
 
 
-(*
- * Regenerate the target object.
- *
- * Any children of the cap are first revoked. The object
- * is then reset into its original (as-if just created)
- * state. But maybe not. It's complex.
- *
- * In the C implementation, attempting to recycle a
- * non-master cap may do something that is not
- * a recycle. (Should be perhaps return an error?)
- *)
-definition
-  clear_object_caps :: "cdl_object_id \<Rightarrow> unit k_monad"
-where
- "clear_object_caps ptr = do
-    ptrs \<leftarrow> gets (\<lambda>s. {cptr. fst cptr = ptr \<and> opt_cap cptr s \<noteq> None});
-    ptrlist \<leftarrow> select {xs. set xs = ptrs \<and> distinct xs};
-    mapM_x empty_slot ptrlist
-  od"
+(* Regenerate the target object.
+
+   Any children of the cap are first revoked. The object is then reset into its original (as if
+   just created) state. But maybe not. It's complex. In the C implementation, attempting to
+   recycle a non-master cap may do something that is not a recycle. *)
+definition clear_object_caps :: "cdl_object_id \<Rightarrow> unit k_monad" where
+  "clear_object_caps ptr = do
+     ptrs \<leftarrow> gets (\<lambda>s. {cptr. fst cptr = ptr \<and> opt_cap cptr s \<noteq> None});
+     ptrlist \<leftarrow> select {xs. set xs = ptrs \<and> distinct xs};
+     mapM_x empty_slot ptrlist
+   od"
 
 definition cdl_default_tcb :: "cdl_object" where
   "cdl_default_tcb \<equiv> Tcb \<lparr>
-    cdl_tcb_caps =
-      [tcb_cspace_slot \<mapsto> cdl_cap.NullCap,
+     cdl_tcb_caps = [
+       tcb_cspace_slot \<mapsto> cdl_cap.NullCap,
        tcb_vspace_slot \<mapsto> cdl_cap.NullCap,
        tcb_replycap_slot \<mapsto> cdl_cap.NullCap,
        tcb_caller_slot \<mapsto> cdl_cap.NullCap,
@@ -488,201 +386,172 @@ definition cdl_default_tcb :: "cdl_object" where
        tcb_pending_op_slot \<mapsto> cdl_cap.NullCap,
        tcb_boundntfn_slot \<mapsto> cdl_cap.NullCap,
        tcb_boundvcpu_slot \<mapsto> cdl_cap.NullCap],
-    cdl_tcb_fault_endpoint = 0,
-    cdl_tcb_intent = \<lparr>
-      cdl_intent_op = None,
-      cdl_intent_error = False,
-      cdl_intent_cap = 0,
-      cdl_intent_extras = [],
-      cdl_intent_recv_slot = None
-    \<rparr>,
-    cdl_tcb_has_fault = False,
-    cdl_tcb_domain = minBound,
-    cdl_tcb_extra = default_tcb_extra_data\<rparr>"
+     cdl_tcb_fault_endpoint = 0,
+     cdl_tcb_intent = \<lparr>
+       cdl_intent_op = None,
+       cdl_intent_error = False,
+       cdl_intent_cap = 0,
+       cdl_intent_extras = [],
+       cdl_intent_recv_slot = None\<rparr>,
+     cdl_tcb_has_fault = False,
+     cdl_tcb_domain = minBound,
+     cdl_tcb_extra = default_tcb_extra_data\<rparr>"
 
-definition obj_tcb :: "cdl_object \<Rightarrow> cdl_tcb"
-where "obj_tcb obj \<equiv> case obj of Tcb tcb \<Rightarrow> tcb"
+definition obj_tcb :: "cdl_object \<Rightarrow> cdl_tcb" where
+  "obj_tcb obj \<equiv> case obj of Tcb tcb \<Rightarrow> tcb"
 
-definition tcb_caps_merge :: "cdl_tcb \<Rightarrow> cdl_tcb \<Rightarrow> cdl_tcb"
-  where "tcb_caps_merge regtcb captcb \<equiv> regtcb\<lparr>cdl_tcb_caps
-  := (cdl_tcb_caps captcb)(tcb_pending_op_slot \<mapsto> the (cdl_tcb_caps regtcb tcb_pending_op_slot), tcb_boundntfn_slot \<mapsto> the (cdl_tcb_caps regtcb tcb_boundntfn_slot))\<rparr>"
+definition tcb_caps_merge :: "cdl_tcb \<Rightarrow> cdl_tcb \<Rightarrow> cdl_tcb" where
+  "tcb_caps_merge regtcb captcb \<equiv>
+     regtcb\<lparr>cdl_tcb_caps :=
+              (cdl_tcb_caps captcb)
+                (tcb_pending_op_slot \<mapsto> the (cdl_tcb_caps regtcb tcb_pending_op_slot),
+                 tcb_boundntfn_slot \<mapsto> the (cdl_tcb_caps regtcb tcb_boundntfn_slot))\<rparr>"
 
-definition merge_with_dft_tcb :: "cdl_object_id \<Rightarrow> unit k_monad"
-where "merge_with_dft_tcb o_id \<equiv>
- do
-  new_intent \<leftarrow> select UNIV;
-  KHeap_D.update_thread o_id (cdl_tcb_intent_update (\<lambda>x. new_intent) \<circ> (tcb_caps_merge (obj_tcb cdl_default_tcb)))
- od"
+definition merge_with_dft_tcb :: "cdl_object_id \<Rightarrow> unit k_monad" where
+  "merge_with_dft_tcb o_id \<equiv> do
+     new_intent \<leftarrow> select UNIV;
+     update_thread o_id
+       (cdl_tcb_intent_update (\<lambda>x. new_intent) \<circ> tcb_caps_merge (obj_tcb cdl_default_tcb))
+   od"
 
-fun
-  reset_mem_mapping :: "cdl_cap \<Rightarrow> cdl_cap"
-where
-  "reset_mem_mapping (FrameCap dev p rts sz b mp) = FrameCap dev p rts sz b None"
-| "reset_mem_mapping (PageTableCap l ptr b mp) = PageTableCap l ptr b None"
-| "reset_mem_mapping cap = cap"
+fun reset_mem_mapping :: "cdl_cap \<Rightarrow> cdl_cap" where
+    "reset_mem_mapping (FrameCap dev p rts sz b mp) = FrameCap dev p rts sz b None"
+  | "reset_mem_mapping (PageTableCap l ptr b mp) = PageTableCap l ptr b None"
+  | "reset_mem_mapping cap = cap"
 
 
-(*
- * Walk a user's CSpace to convert a user's CPTR into a cap slot.
- *)
-function
-  resolve_address_bits ::
+(* Walk a user's CSpace to convert a user's CPTR into a cap slot. *)
+function resolve_address_bits ::
   "cdl_cap \<Rightarrow> cdl_cptr \<Rightarrow> nat \<Rightarrow> (cdl_cap_ref \<times> nat) fault_monad"
-where
+  where
   "resolve_address_bits cnode_cap cap_ptr remaining_size = doE
-    unlessE (is_cnode_cap cnode_cap) $ throw;
+     unlessE (is_cnode_cap cnode_cap) $ throw;
 
-    \<comment> \<open>Fetch the next level CNode.\<close>
-    cnode \<leftarrow> liftE $ get_cnode $ cap_object cnode_cap;
-    radix_size \<leftarrow> returnOk $ cdl_cnode_size_bits cnode;
-    guard_size \<leftarrow> returnOk $ cap_guard_size cnode_cap;
-    cap_guard  \<leftarrow> returnOk $ cap_guard cnode_cap;
-    level_size \<leftarrow> returnOk (radix_size + guard_size);
-    assertE (level_size \<noteq> 0);
+     \<comment> \<open>Fetch the next level CNode.\<close>
+     cnode \<leftarrow> liftE $ get_cnode $ cap_object cnode_cap;
+     radix_size \<leftarrow> returnOk $ cdl_cnode_size_bits cnode;
+     guard_size \<leftarrow> returnOk $ cap_guard_size cnode_cap;
+     cap_guard  \<leftarrow> returnOk $ cap_guard cnode_cap;
+     level_size \<leftarrow> returnOk (radix_size + guard_size);
+     assertE (level_size \<noteq> 0);
 
-    \<comment> \<open>Ensure the guard matches up.\<close>
-    guard \<leftarrow> returnOk $ (cap_ptr >> (remaining_size-guard_size)) && (mask guard_size);
-    unlessE (guard_size \<le> remaining_size \<and> guard = cap_guard) $ throw;
+     \<comment> \<open>Ensure the guard matches up.\<close>
+     guard \<leftarrow> returnOk $ (cap_ptr >> (remaining_size-guard_size)) && (mask guard_size);
+     unlessE (guard_size \<le> remaining_size \<and> guard = cap_guard) $ throw;
 
-    \<comment> \<open>Ensure we still enough unresolved bits left in our CPTR.\<close>
-    whenE (level_size > remaining_size) $ throw;
+     \<comment> \<open>Ensure we still enough unresolved bits left in our CPTR.\<close>
+     whenE (level_size > remaining_size) $ throw;
 
-    \<comment> \<open>Find the next slot.\<close>
-    offset \<leftarrow> returnOk $ (cap_ptr >> (remaining_size-level_size)) && (mask radix_size);
-    slot \<leftarrow> returnOk (cap_object cnode_cap, unat offset);
-    size_left \<leftarrow> returnOk (remaining_size - level_size);
-    if (size_left = 0) then
-      returnOk (slot, 0)
-    else
-      doE
-        next_cap \<leftarrow> liftE $ get_cap (slot);
-        if is_cnode_cap next_cap then
-          resolve_address_bits next_cap cap_ptr size_left
-        else
-          returnOk (slot, size_left)
-      odE
-  odE"
+     \<comment> \<open>Find the next slot.\<close>
+     offset \<leftarrow> returnOk $ (cap_ptr >> (remaining_size-level_size)) && (mask radix_size);
+      slot \<leftarrow> returnOk (cap_object cnode_cap, unat offset);
+     size_left \<leftarrow> returnOk (remaining_size - level_size);
+     if size_left = 0 then
+       returnOk (slot, 0)
+     else doE
+       next_cap \<leftarrow> liftE $ get_cap (slot);
+       if is_cnode_cap next_cap
+       then resolve_address_bits next_cap cap_ptr size_left
+       else returnOk (slot, size_left)
+     odE
+   odE"
   by fastforce+
 
 termination resolve_address_bits
-  apply (relation "measure (\<lambda>(a,b,c). c)")
-  apply (auto simp: in_monad)
-  done
+  by (relation "measure (\<lambda>(a,b,c). c)") (auto simp: in_monad)
 
-definition
-  lookup_slot :: "cdl_object_id \<Rightarrow> cdl_cptr \<Rightarrow> cdl_cap_ref fault_monad"
-where
-  "lookup_slot thread cptr \<equiv>
-    doE
-      cspace_root \<leftarrow> liftE $ get_cap (thread, tcb_cspace_slot);
-      (slot, _) \<leftarrow> resolve_address_bits cspace_root cptr word_bits;
-      returnOk slot
-    odE"
+definition lookup_slot :: "cdl_object_id \<Rightarrow> cdl_cptr \<Rightarrow> cdl_cap_ref fault_monad" where
+  "lookup_slot thread cptr \<equiv> doE
+     cspace_root \<leftarrow> liftE $ get_cap (thread, tcb_cspace_slot);
+     (slot, _) \<leftarrow> resolve_address_bits cspace_root cptr word_bits;
+     returnOk slot
+   odE"
 
-definition
-  lookup_cap :: "cdl_object_id \<Rightarrow> cdl_cptr \<Rightarrow> cdl_cap fault_monad"
-where
-  "lookup_cap thread cptr \<equiv>
-    doE
-      slot \<leftarrow> lookup_slot thread cptr;
-      liftE $ get_cap slot
-    odE"
+definition lookup_cap :: "cdl_object_id \<Rightarrow> cdl_cptr \<Rightarrow> cdl_cap fault_monad" where
+  "lookup_cap thread cptr \<equiv> doE
+     slot \<leftarrow> lookup_slot thread cptr;
+     liftE $ get_cap slot
+   odE"
 
-definition
-  lookup_cap_and_slot :: "cdl_object_id \<Rightarrow> cdl_cptr \<Rightarrow> (cdl_cap \<times> cdl_cap_ref) fault_monad"
-where
-  "lookup_cap_and_slot thread cptr \<equiv>
-    doE
-      slot \<leftarrow> lookup_slot thread cptr;
-      cap \<leftarrow> liftE $ get_cap slot;
-      returnOk (cap, slot)
-    odE"
+definition lookup_cap_and_slot ::
+  "cdl_object_id \<Rightarrow> cdl_cptr \<Rightarrow> (cdl_cap \<times> cdl_cap_ref) fault_monad"
+  where
+  "lookup_cap_and_slot thread cptr \<equiv> doE
+     slot \<leftarrow> lookup_slot thread cptr;
+     cap \<leftarrow> liftE $ get_cap slot;
+     returnOk (cap, slot)
+   odE"
 
-definition
-  lookup_slot_for_cnode_op :: "cdl_cap \<Rightarrow> cdl_cptr \<Rightarrow> nat \<Rightarrow> cdl_cap_ref except_monad"
-where
-  "lookup_slot_for_cnode_op croot cptr depth \<equiv>
-    doE
-      whenE (depth < 1 \<or> depth > word_bits) throw;
-      (slot, rem) \<leftarrow> fault_to_except $ resolve_address_bits croot cptr depth;
-      if rem = 0 then returnOk slot else throw
-    odE"
+definition lookup_slot_for_cnode_op :: "cdl_cap \<Rightarrow> cdl_cptr \<Rightarrow> nat \<Rightarrow> cdl_cap_ref except_monad"
+  where
+  "lookup_slot_for_cnode_op croot cptr depth \<equiv> doE
+     whenE (depth < 1 \<or> depth > word_bits) throw;
+     (slot, rem) \<leftarrow> fault_to_except $ resolve_address_bits croot cptr depth;
+     if rem = 0 then returnOk slot else throw
+   odE"
 
 
-(*
- * Update the badge of a badged cap. For notification and endpoint caps, mask off bits the kernel
- * is unable to store for implementation reasons.
- *)
-definition
-  badge_update :: "machine_word \<Rightarrow> cdl_cap \<Rightarrow> cdl_cap"
-where
+(* Update the badge of a badged cap. For notification and endpoint caps, mask off bits the kernel
+   is unable to store for implementation reasons. *)
+definition badge_update :: "machine_word \<Rightarrow> cdl_cap \<Rightarrow> cdl_cap" where
   "badge_update data cap \<equiv>
      let
        data' = if is_ep_cap cap \<or> is_ntfn_cap cap then data && mask badge_bits else data
      in
        update_cap_badge data' cap"
 
-(*
- * Transform a capability based on a request from the user.
- *
- * The "data" word is interpreted differently for different cap types.
- *
- * We return a set of possible caps to allow for non-deterministic
- * implementations, to avoid messy implementation details of the CDT
- * in lower-level models.
- *)
+(* Transform a capability based on a request from the user.
+
+   The "data" word is interpreted differently for different cap types.
+
+   We return a set of possible caps to allow for non-deterministic
+   implementations, to avoid messy implementation details of the CDT
+   in lower-level models. *)
 definition update_cap_data :: "bool \<Rightarrow> machine_word \<Rightarrow> cdl_cap \<Rightarrow> cdl_cap k_monad" where
   "update_cap_data preserve data cap \<equiv>
-    return $ case cap of
-        EndpointCap _ b _ \<Rightarrow> if b = 0 \<and> \<not> preserve then badge_update data cap else NullCap
-      | NotificationCap _ b _ \<Rightarrow> if b = 0 \<and> \<not> preserve then badge_update data cap else NullCap
-      | CNodeCap object guard guard_size sz \<Rightarrow>
-          let
-            reserved_bits = 3;
-            guard_bits = 18;
-            guard_size_bits = 5;
-            new_guard_size = unat ((data >> reserved_bits) && mask guard_size_bits);
-            new_guard = (data >> (reserved_bits + guard_size_bits)) &&
-                        mask (min (unat ((data >> reserved_bits) && mask guard_size_bits)) guard_bits)
-          in
-            if new_guard_size + sz > word_bits
-            then NullCap
-            else CNodeCap object new_guard new_guard_size sz
-      | SMCCap b \<Rightarrow> if b = 0 \<and> \<not> preserve then badge_update data cap else NullCap
-      | _ \<Rightarrow> cap"
+     return $ case cap of
+       EndpointCap _ b _ \<Rightarrow> if b = 0 \<and> \<not> preserve then badge_update data cap else NullCap
+     | NotificationCap _ b _ \<Rightarrow> if b = 0 \<and> \<not> preserve then badge_update data cap else NullCap
+     | CNodeCap object guard guard_size sz \<Rightarrow>
+         let
+           reserved_bits = 3;
+           guard_bits = 18;
+           guard_size_bits = 5;
+           new_guard_size = unat ((data >> reserved_bits) && mask guard_size_bits);
+           new_guard = (data >> (reserved_bits + guard_size_bits)) &&
+                       mask (min (unat ((data >> reserved_bits) && mask guard_size_bits)) guard_bits)
+         in
+           if new_guard_size + sz > word_bits
+           then NullCap
+           else CNodeCap object new_guard new_guard_size sz
+     | SMCCap b \<Rightarrow> if b = 0 \<and> \<not> preserve then badge_update data cap else NullCap
+     | _ \<Rightarrow> cap"
 
-(*
- * Some caps may not be copied/minted. In this case the following function
- * returns NullCap or throws.
- *
- * PageTable and PageDirectory caps may not be copied if already mapped. This is
- * left out here and modelled by nondeterminism.
- *)
-definition
-  derive_cap :: "cdl_cap_ref \<Rightarrow> cdl_cap \<Rightarrow> cdl_cap except_monad"
-where
-  "derive_cap slot cap \<equiv> case cap of
-     UntypedCap _ _ _ \<Rightarrow> doE ensure_no_children slot; returnOk cap odE
-   | ReplyCap _ _ \<Rightarrow> returnOk NullCap
-   | MasterReplyCap oref \<Rightarrow> returnOk NullCap
-   | IrqControlCap \<Rightarrow> returnOk NullCap
-   | ZombieCap _ \<Rightarrow> returnOk NullCap
-   | FrameCap dev p r sz b x \<Rightarrow> returnOk (FrameCap dev p r sz b None)
-   | PageTableCap _ _ _ _ \<Rightarrow> throw \<sqinter> returnOk cap
-   | _ \<Rightarrow> returnOk cap"
+(* Some caps may not be copied/minted. In this case the following function
+   returns NullCap or throws.
+
+   PageTable and PageDirectory caps may not be copied if already mapped. This is
+   left out here and modelled by nondeterminism. *)
+definition derive_cap :: "cdl_cap_ref \<Rightarrow> cdl_cap \<Rightarrow> cdl_cap except_monad" where
+  "derive_cap slot cap \<equiv>
+     case cap of
+       UntypedCap _ _ _        \<Rightarrow> doE ensure_no_children slot; returnOk cap odE
+     | ReplyCap _ _            \<Rightarrow> returnOk NullCap
+     | MasterReplyCap oref     \<Rightarrow> returnOk NullCap
+     | IrqControlCap           \<Rightarrow> returnOk NullCap
+     | ZombieCap _             \<Rightarrow> returnOk NullCap
+     | FrameCap dev p r sz b x \<Rightarrow> returnOk (FrameCap dev p r sz b None)
+     | PageTableCap _ _ _ _    \<Rightarrow> throw \<sqinter> returnOk cap
+     | _                       \<Rightarrow> returnOk cap"
 
 
-(* This function is here to make it available in both Tcb_D and
-   PageTable_D *)
+(* This function is here to make it available in both Tcb_D and PageTable_D *)
 
 (* Modify the TCB's IpcBuffer or Registers in an arbitrary fashion. *)
-definition
-  corrupt_tcb_intent :: "cdl_object_id \<Rightarrow> unit k_monad"
-where
-  "corrupt_tcb_intent target_tcb \<equiv>
-    do
-      new_intent \<leftarrow> select UNIV;
-      update_thread target_tcb (\<lambda>t. t\<lparr>cdl_tcb_intent := new_intent\<rparr>)
-    od"
+definition corrupt_tcb_intent :: "cdl_object_id \<Rightarrow> unit k_monad" where
+  "corrupt_tcb_intent target_tcb \<equiv> do
+     new_intent \<leftarrow> select UNIV;
+     update_thread target_tcb (\<lambda>t. t\<lparr>cdl_tcb_intent := new_intent\<rparr>)
+   od"
 
 end
