spec/capDL/Endpoint_D.thy
@@ -4,475 +4,373 @@
  * SPDX-License-Identifier: GPL-2.0-only
  *)
 
-(*
- * Operations on endpoints.
- *)
+(* Operations on endpoints.  *)
 
 theory Endpoint_D
-imports Invocations_D CSpace_D Tcb_D
+  imports
+    Invocations_D
+    CSpace_D
+    Tcb_D
 begin
 
 (* Inject the reply cap into the target TCB *)
-definition
-  inject_reply_cap :: "cdl_object_id \<Rightarrow> cdl_object_id \<Rightarrow> bool \<Rightarrow> unit k_monad"
-where
+definition inject_reply_cap :: "cdl_object_id \<Rightarrow> cdl_object_id \<Rightarrow> bool \<Rightarrow> unit k_monad" where
   "inject_reply_cap src_tcb_id dst_tcb_id can_grant \<equiv> do
-     set_cap (src_tcb_id, tcb_pending_op_slot) $
-         cdl_cap.PendingSyncRecvCap src_tcb_id True False;
+     set_cap (src_tcb_id, tcb_pending_op_slot) $ PendingSyncRecvCap src_tcb_id True False;
      insert_cap_child (ReplyCap src_tcb_id (if can_grant then {Grant, Write} else {Write}))
                       (src_tcb_id, tcb_replycap_slot)
                       (dst_tcb_id, tcb_caller_slot);
      return ()
-  od"
-
-(*
- * Get the slot where we should place an incoming cap for a
- * particular thread.
- *)
-
-definition
-  get_receive_slot :: "cdl_object_id \<Rightarrow> cdl_cap_ref option k_monad"
-where
-  "get_receive_slot thread \<equiv>
-    do
-      tcb \<leftarrow> get_thread thread;
-      recv_slot \<leftarrow> (case (cdl_tcb_caps tcb tcb_ipcbuffer_slot) of (Some (FrameCap _ _ rights _ _ _)) \<Rightarrow>
-        if (Read \<in> rights \<and> Write \<in> rights)
-          then return (cdl_intent_recv_slot (cdl_tcb_intent tcb))
-        else
-          return None
-      | _ \<Rightarrow> return None);
-      case ( recv_slot ) of
-          None \<Rightarrow>
-            return None
-        | Some (croot, index, depth) \<Rightarrow>
-            doE
-              \<comment> \<open>Lookup the slot.\<close>
-              cspace_root \<leftarrow> unify_failure $ lookup_cap thread croot;
-              result \<leftarrow> unify_failure $ lookup_slot_for_cnode_op cspace_root index depth;
-
-              \<comment> \<open>Ensure nothing is already in it.\<close>
-              cap \<leftarrow> liftE $ get_cap result;
-              whenE (cap \<noteq> NullCap) throw;
-
-              returnOk $ Some result
-            odE <catch> (\<lambda>_. return None)
-    od
-  "
-
-(* Get the cptr's that the given thread wishes to transfer. *)
-definition
-  get_send_slots :: "cdl_object_id \<Rightarrow> cdl_cptr list k_monad"
-where
-  "get_send_slots thread \<equiv>
-    do
-      tcb \<leftarrow> get_thread thread;
-      return $ cdl_intent_extras (cdl_tcb_intent tcb)
-    od
-  "
-
-definition
-  get_ipc_buffer :: "cdl_object_id \<Rightarrow> bool \<Rightarrow> cdl_object_id option k_monad"
-where
-  "get_ipc_buffer oid in_receive \<equiv> do
-    frame_cap \<leftarrow> get_cap (oid,tcb_ipcbuffer_slot);
-    (case frame_cap of
-        Types_D.FrameCap _ a rights _ _ _ \<Rightarrow> if (Write \<in> rights \<and> Read \<in> rights) \<or> (Read\<in> rights \<and> \<not> in_receive)
-          then return (Some a)
-          else return None
-        | _ \<Rightarrow> return None)
    od"
 
-definition
-  corrupt_ipc_buffer :: "cdl_object_id \<Rightarrow> bool \<Rightarrow> unit k_monad"
-  where
+(* Get the slot where we should place an incoming cap for a particular thread. *)
+definition get_receive_slot :: "cdl_object_id \<Rightarrow> cdl_cap_ref option k_monad" where
+  "get_receive_slot thread \<equiv> do
+     tcb \<leftarrow> get_thread thread;
+     recv_slot \<leftarrow> case cdl_tcb_caps tcb tcb_ipcbuffer_slot of
+                    Some (FrameCap _ _ rights _ _ _) \<Rightarrow>
+                      if Read \<in> rights \<and> Write \<in> rights
+                      then return (cdl_intent_recv_slot (cdl_tcb_intent tcb))
+                      else return None
+                  | _ \<Rightarrow> return None;
+     case recv_slot of
+       None \<Rightarrow> return None
+     | Some (croot, index, depth) \<Rightarrow> doE
+       \<comment> \<open>Lookup the slot.\<close>
+       cspace_root \<leftarrow> unify_failure $ lookup_cap thread croot;
+       result \<leftarrow> unify_failure $ lookup_slot_for_cnode_op cspace_root index depth;
+
+       \<comment> \<open>Ensure nothing is already in it.\<close>
+       cap \<leftarrow> liftE $ get_cap result;
+       whenE (cap \<noteq> NullCap) throw;
+
+       returnOk $ Some result
+     odE <catch> (\<lambda>_. return None)
+   od"
+
+(* Get the cptr's that the given thread wishes to transfer. *)
+definition get_send_slots :: "cdl_object_id \<Rightarrow> cdl_cptr list k_monad" where
+  "get_send_slots thread \<equiv> do
+     tcb \<leftarrow> get_thread thread;
+     return $ cdl_intent_extras (cdl_tcb_intent tcb)
+   od"
+
+definition get_ipc_buffer :: "cdl_object_id \<Rightarrow> bool \<Rightarrow> cdl_object_id option k_monad" where
+  "get_ipc_buffer oid in_receive \<equiv> do
+     frame_cap \<leftarrow> get_cap (oid, tcb_ipcbuffer_slot);
+     case frame_cap of
+        FrameCap _ a rights _ _ _ \<Rightarrow>
+          if (Write \<in> rights \<and> Read \<in> rights) \<or> (Read \<in> rights \<and> \<not>in_receive)
+          then return (Some a)
+          else return None
+        | _ \<Rightarrow> return None
+   od"
+
+definition corrupt_ipc_buffer :: "cdl_object_id \<Rightarrow> bool \<Rightarrow> unit k_monad" where
   "corrupt_ipc_buffer oid in_receive \<equiv> do
-    buffer \<leftarrow> get_ipc_buffer oid in_receive;
-    (case buffer of
-        Some a \<Rightarrow> corrupt_frame a
-      | None \<Rightarrow> corrupt_tcb_intent oid)
-  od"
+     buffer \<leftarrow> get_ipc_buffer oid in_receive;
+     case buffer of
+       Some a \<Rightarrow> corrupt_frame a
+     | None \<Rightarrow> corrupt_tcb_intent oid
+   od"
 
-(*
- * Transfers at most one cap in addition to a number of endpoint badges.
- *
- * Endpoint badges are transferred if the cap to be transferred is to
- * the endpoint used in the transfer.
- *)
-fun
-  transfer_caps_loop :: "cdl_object_id option \<Rightarrow> cdl_object_id \<Rightarrow>
-                         (cdl_cap \<times> cdl_cap_ref) list \<Rightarrow> cdl_cap_ref option
-                         \<Rightarrow> unit k_monad"
-where
-  "transfer_caps_loop ep receiver [] dest = return ()"
-| "transfer_caps_loop ep receiver ((cap,slot)#caps) dest =
-      \<comment> \<open>Transfer badge, transfer cap, or abort early if more than
-         one cap to transfer\<close>
-      (if is_ep_cap cap \<and> ep = Some (cap_object cap)
-      then do
-        \<comment> \<open>transfer badge\<close>
-        corrupt_ipc_buffer receiver True;
-        \<comment> \<open>transfer rest of badges or cap\<close>
-        transfer_caps_loop ep receiver caps dest
-      od
-      else if dest \<noteq> None then doE
-        new_cap \<leftarrow> returnOk (update_cap_rights (cap_rights cap - {Write}) cap) \<sqinter>
-                  returnOk cap;
+(* Transfers at most one cap in addition to a number of endpoint badges.
 
-        \<comment> \<open>Target cap is derived. This may abort transfer early.\<close>
-        target_cap \<leftarrow> derive_cap slot new_cap;
-        whenE (target_cap = NullCap) throw;
+   Endpoint badges are transferred if the cap to be transferred is to
+   the endpoint used in the transfer. *)
+fun transfer_caps_loop ::
+  "cdl_object_id option \<Rightarrow> cdl_object_id \<Rightarrow> (cdl_cap \<times> cdl_cap_ref) list \<Rightarrow> cdl_cap_ref option \<Rightarrow>
+   unit k_monad"
+  where
+    "transfer_caps_loop ep receiver [] dest = return ()"
+  | "transfer_caps_loop ep receiver ((cap, slot) # caps) dest =
+       \<comment> \<open>Transfer badge, transfer cap, or abort early if more than one cap to transfer\<close>
+       (if is_ep_cap cap \<and> ep = Some (cap_object cap)
+        then do
+          \<comment> \<open>transfer badge\<close>
+          corrupt_ipc_buffer receiver True;
+          \<comment> \<open>transfer rest of badges or cap\<close>
+          transfer_caps_loop ep receiver caps dest
+        od
+        else if dest \<noteq> None then doE
+          new_cap \<leftarrow> returnOk (update_cap_rights (cap_rights cap - {Write}) cap) \<sqinter>
+                     returnOk cap;
 
-        \<comment> \<open>Copy the cap across as either a child or sibling.\<close>
-        liftE (insert_cap_child target_cap slot (the dest)
-               \<sqinter> insert_cap_sibling target_cap slot (the dest));
+          \<comment> \<open>Target cap is derived. This may abort transfer early.\<close>
+          target_cap \<leftarrow> derive_cap slot new_cap;
+          whenE (target_cap = NullCap) throw;
 
-        \<comment> \<open>Transfer rest of badges\<close>
-        liftE $ transfer_caps_loop ep receiver caps None
-      odE <catch> (\<lambda>_. return ())
-      else
-        return ())"
+          \<comment> \<open>Copy the cap across as either a child or sibling.\<close>
+          liftE (insert_cap_child target_cap slot (the dest)
+                 \<sqinter> insert_cap_sibling target_cap slot (the dest));
+
+          \<comment> \<open>Transfer rest of badges\<close>
+          liftE $ transfer_caps_loop ep receiver caps None
+        odE <catch> (\<lambda>_. return ())
+        else return ())"
 
 
-(*
- * Transfer caps from src to dest.
- *
- * In theory, the source thread specifies a list of caps to send, and
- * the destination thread specifies a list of cap slots to put them in.
- *
- * In the true spirit of L4 Pistachio, what _actually_ occurs during the
- * IPC transfer is hard to determine without knowing intricate details
- * of the kernel's implementation. In particular:
- *
- *   - Caps often just won't send, but still 'burn' the receive slot
- *     (ZombieCaps, ReplyCaps, IrqControlCap);
- *
- *   - Caps may not send, but still allow later caps to
- *     use the receive slot (Unwrapped endpoints);
- *
- *   - Cap sending may stop half way (cap lookup faults);
- *
- *   - The new cap may either be a sibling or child of source cap,
- *     depending on where in the CDT the source cap is.
- *
- *   - In reality, no more than one cap will ever be sent, because only
- *     one destination cap slot is supported elsewhere in the code.
- *
- * We remove some of the details, replacing them with nondeterminism.
- *)
-definition
-  transfer_caps :: "cdl_object_id option \<Rightarrow> (cdl_cap \<times> cdl_cap_ref) list \<Rightarrow>
-                    cdl_object_id \<Rightarrow> cdl_object_id \<Rightarrow> unit k_monad"
-where
-  "transfer_caps ep caps sender receiver \<equiv>
-    do
-      dest_slot \<leftarrow> get_receive_slot receiver \<sqinter> return None;
-      transfer_caps_loop ep receiver caps dest_slot
-    od"
+(* Transfer caps from src to dest.
 
-(*
- * Get the set of threads waiting to receive on the given notification.
- *)
-definition
-  get_waiting_ntfn_recv_threads :: "cdl_object_id \<Rightarrow> cdl_state \<Rightarrow> cdl_object_id set"
-where
+   In theory, the source thread specifies a list of caps to send, and
+   the destination thread specifies a list of cap slots to put them in.
+
+   In the true spirit of L4 Pistachio, what _actually_ occurs during the
+   IPC transfer is hard to determine without knowing intricate details
+   of the kernel's implementation. In particular:
+
+    - Caps often just won't send, but still 'burn' the receive slot
+      (ZombieCaps, ReplyCaps, IrqControlCap);
+
+    - Caps may not send, but still allow later caps to
+      use the receive slot (Unwrapped endpoints);
+
+    - Cap sending may stop half way (cap lookup faults);
+
+    - The new cap may either be a sibling or child of source cap,
+      depending on where in the CDT the source cap is.
+
+    - In reality, no more than one cap will ever be sent, because only
+      one destination cap slot is supported elsewhere in the code.
+
+  We remove some of the details, replacing them with nondeterminism. *)
+definition transfer_caps ::
+  "cdl_object_id option \<Rightarrow> (cdl_cap \<times> cdl_cap_ref) list \<Rightarrow> cdl_object_id \<Rightarrow> cdl_object_id \<Rightarrow>
+   unit k_monad"
+  where
+  "transfer_caps ep caps sender receiver \<equiv> do
+     dest_slot \<leftarrow> get_receive_slot receiver \<sqinter> return None;
+     transfer_caps_loop ep receiver caps dest_slot
+   od"
+
+(* Get the set of threads waiting to receive on the given notification. *)
+definition get_waiting_ntfn_recv_threads :: "cdl_object_id \<Rightarrow> cdl_state \<Rightarrow> cdl_object_id set" where
   "get_waiting_ntfn_recv_threads target state \<equiv>
-     {x. \<exists>a. (cdl_objects state) x = Some (Tcb a) \<and>
-         (((cdl_tcb_caps a) tcb_pending_op_slot) = Some (PendingNtfnRecvCap target)) }"
+     {x. \<exists>a. cdl_objects state x = Some (Tcb a) \<and>
+             cdl_tcb_caps a tcb_pending_op_slot = Some (PendingNtfnRecvCap target)}"
 
 (* Get the set of threads waiting to receive on the given sync endpoint. *)
-definition
-  get_waiting_sync_recv_threads :: "cdl_object_id \<Rightarrow> cdl_state \<Rightarrow> cdl_object_id set"
-where
+definition get_waiting_sync_recv_threads :: "cdl_object_id \<Rightarrow> cdl_state \<Rightarrow> cdl_object_id set" where
   "get_waiting_sync_recv_threads target state \<equiv>
-     {x. \<exists>a. (cdl_objects state) x = Some (Tcb a) \<and>
-         (\<exists>can_grant. (cdl_tcb_caps a) tcb_pending_op_slot = Some (PendingSyncRecvCap target False can_grant)) }"
+     {x. \<exists>a. cdl_objects state x = Some (Tcb a) \<and>
+              (\<exists>can_grant. cdl_tcb_caps a tcb_pending_op_slot =
+                             Some (PendingSyncRecvCap target False can_grant))}"
 
-(*
- * Get the set of threads waiting to send to the given sync endpoint.
- *)
-definition
-  get_waiting_sync_send_threads :: "cdl_object_id \<Rightarrow> cdl_state \<Rightarrow> cdl_object_id set"
-where
+(* Get the set of threads waiting to send to the given sync endpoint. *)
+definition get_waiting_sync_send_threads :: "cdl_object_id \<Rightarrow> cdl_state \<Rightarrow> cdl_object_id set" where
   "get_waiting_sync_send_threads target state \<equiv>
-     {t. \<exists>fault a b. (cdl_objects state) t = Some (Tcb a) \<and>
-         (\<exists>call can_grant can_grant_reply. (cdl_tcb_caps a) tcb_pending_op_slot =
-                    Some (PendingSyncSendCap target b call can_grant can_grant_reply fault)) }"
+     {t. \<exists>fault a b. cdl_objects state t = Some (Tcb a) \<and>
+         (\<exists>call can_grant can_grant_reply.
+            cdl_tcb_caps a tcb_pending_op_slot =
+              Some (PendingSyncSendCap target b call can_grant can_grant_reply fault))}"
 
-(*
- * Get the set of threads which are bound to the given ntfn, but are
- * also waiting on sync IPC
- *)
-definition
-  get_waiting_sync_bound_ntfn_threads :: "cdl_object_id \<Rightarrow> cdl_state \<Rightarrow> cdl_object_id set"
-where
+(* Get the set of threads which are bound to the given ntfn, but are  also waiting on sync IPC *)
+definition get_waiting_sync_bound_ntfn_threads :: "cdl_object_id \<Rightarrow> cdl_state \<Rightarrow> cdl_object_id set"
+  where
   "get_waiting_sync_bound_ntfn_threads ntfn_id state \<equiv>
-     {x. \<exists>a ep_id. (cdl_objects state) x = Some (Tcb a) \<and>
-         (\<exists>can_grant. (cdl_tcb_caps a) tcb_pending_op_slot = Some (PendingSyncRecvCap ep_id False can_grant)) \<and>
-         ((cdl_tcb_caps a) tcb_boundntfn_slot = Some (BoundNotificationCap ntfn_id))}"
+     {x. \<exists>a ep_id. cdl_objects state x = Some (Tcb a) \<and>
+                   (\<exists>can_grant. cdl_tcb_caps a tcb_pending_op_slot =
+                                  Some (PendingSyncRecvCap ep_id False can_grant)) \<and>
+                   cdl_tcb_caps a tcb_boundntfn_slot = Some (BoundNotificationCap ntfn_id)}"
 
-(*
- * Mark a thread blocked on IPC.
- *
- * Theads get a new implicit "send once" or "receive once" capability
- * when they block on an IPC. This is because if the capability they
- * used to start the send/receive is revoked, the transfer will still be
- * allowed to proceed (even if it is at a much later point in time).
- *)
+(* Mark a thread blocked on IPC.
 
-definition
-  block_thread_on_ipc :: "cdl_object_id \<Rightarrow> cdl_cap \<Rightarrow> unit k_monad"
-where
-  "block_thread_on_ipc tcb cap \<equiv> set_cap (tcb, tcb_pending_op_slot) cap" (* Might need to do some check here *)
+   Theads get a new implicit "send once" or "receive once" capability
+   when they block on an IPC. This is because if the capability they
+   used to start the send/receive is revoked, the transfer will still be
+   allowed to proceed (even if it is at a much later point in time). *)
+definition block_thread_on_ipc :: "cdl_object_id \<Rightarrow> cdl_cap \<Rightarrow> unit k_monad" where
+  "block_thread_on_ipc tcb cap \<equiv> set_cap (tcb, tcb_pending_op_slot) cap"
 
-definition
-  lookup_extra_caps :: "cdl_object_id \<Rightarrow> cdl_cptr list \<Rightarrow> (cdl_cap \<times> cdl_cap_ref) list fault_monad"
-where
-  "lookup_extra_caps thread cptrs \<equiv>
-     mapME (\<lambda>cptr. lookup_cap_and_slot thread cptr) cptrs"
+definition lookup_extra_caps ::
+  "cdl_object_id \<Rightarrow> cdl_cptr list \<Rightarrow> (cdl_cap \<times> cdl_cap_ref) list fault_monad"
+  where
+  "lookup_extra_caps thread cptrs \<equiv> mapME (\<lambda>cptr. lookup_cap_and_slot thread cptr) cptrs"
 
-(*
- * Transfer a message from "sender" to "receiver", possibly copying caps
- * over in the process. If a fault is pending in receiver, send fault instead.
- *)
-definition
-  do_ipc_transfer :: "cdl_object_id option \<Rightarrow> cdl_object_id \<Rightarrow> cdl_object_id \<Rightarrow> bool \<Rightarrow> unit k_monad"
-where
+(* Transfer a message from "sender" to "receiver", possibly copying caps
+   over in the process. If a fault is pending in receiver, send fault instead. *)
+definition do_ipc_transfer ::
+  "cdl_object_id option \<Rightarrow> cdl_object_id \<Rightarrow> cdl_object_id \<Rightarrow> bool \<Rightarrow> unit k_monad"
+  where
   "do_ipc_transfer ep_id sender_id receiver_id can_grant \<equiv> do
-      \<comment> \<open>look up cap transfer\<close>
-      src_slots \<leftarrow> get_send_slots sender_id;
-      do \<comment> \<open>do normal transfer\<close>
-        caps \<leftarrow> if can_grant then
-                lookup_extra_caps sender_id src_slots <catch> (\<lambda>_. return [])
-              else
-                return [];
-        \<comment> \<open>copy registers, transfer message or fault\<close>
-        corrupt_ipc_buffer receiver_id True;
-        \<comment> \<open>transfer caps if no fault occured\<close>
-        transfer_caps ep_id caps sender_id receiver_id
-      od  \<sqinter>  \<comment> \<open>fault transfer\<close>
-      corrupt_ipc_buffer receiver_id True;
-      \<comment> \<open>set message info\<close>
-      corrupt_tcb_intent receiver_id
-  od"
+     \<comment> \<open>look up cap transfer\<close>
+     src_slots \<leftarrow> get_send_slots sender_id;
+     do \<comment> \<open>do normal transfer\<close>
+       caps \<leftarrow> if can_grant
+               then lookup_extra_caps sender_id src_slots <catch> (\<lambda>_. return [])
+               else return [];
+       \<comment> \<open>copy registers, transfer message or fault\<close>
+       corrupt_ipc_buffer receiver_id True;
+       \<comment> \<open>transfer caps if no fault occured\<close>
+       transfer_caps ep_id caps sender_id receiver_id
+     od \<sqinter>
+     \<comment> \<open>fault transfer\<close>
+     corrupt_ipc_buffer receiver_id True;
+     \<comment> \<open>set message info\<close>
+     corrupt_tcb_intent receiver_id
+   od"
 
+(* Transfer a message from "sender" to "receiver" using a reply capability.
 
-(*
- * Transfer a message from "sender" to "receiver" using a reply capability.
- *
- * The sender may have the right to grant caps over the channel.
- *
- * If a fault is pending in the receiver, the fault is transferred.
- *)
-
-definition
-  do_reply_transfer :: "cdl_object_id \<Rightarrow> cdl_object_id \<Rightarrow> cdl_cap_ref \<Rightarrow> bool \<Rightarrow> unit k_monad"
-where
-  "do_reply_transfer sender_id receiver_id reply_cap_slot can_grant \<equiv>
-    do
-      has_fault \<leftarrow> get_thread_fault receiver_id;
-      when (\<not> has_fault) $ do_ipc_transfer None sender_id receiver_id can_grant;
-      \<comment> \<open>Clear out any pending operation caps.\<close>
-      delete_cap_simple reply_cap_slot;
-      when (has_fault) $ (do corrupt_tcb_intent receiver_id;
-        update_thread_fault receiver_id (\<lambda>_. False) od );
-      if ( \<not> has_fault) then set_cap (receiver_id, tcb_pending_op_slot) RunningCap
-      else
-         (set_cap (receiver_id,tcb_pending_op_slot) NullCap
-        \<sqinter> set_cap (receiver_id,tcb_pending_op_slot) RestartCap)
+   The sender may have the right to grant caps over the channel. If a fault is pending in the
+   receiver, the fault is transferred. *)
+definition do_reply_transfer ::
+  "cdl_object_id \<Rightarrow> cdl_object_id \<Rightarrow> cdl_cap_ref \<Rightarrow> bool \<Rightarrow> unit k_monad"
+  where
+  "do_reply_transfer sender_id receiver_id reply_cap_slot can_grant \<equiv> do
+     has_fault \<leftarrow> get_thread_fault receiver_id;
+     when (\<not>has_fault) $ do_ipc_transfer None sender_id receiver_id can_grant;
+     \<comment> \<open>Clear out any pending operation caps.\<close>
+     delete_cap_simple reply_cap_slot;
+     when has_fault $ do
+       corrupt_tcb_intent receiver_id;
+       update_thread_fault receiver_id (\<lambda>_. False)
+     od;
+     if \<not>has_fault
+     then set_cap (receiver_id, tcb_pending_op_slot) RunningCap
+     else (set_cap (receiver_id,tcb_pending_op_slot) NullCap \<sqinter>
+           set_cap (receiver_id,tcb_pending_op_slot) RestartCap)
     od"
 
 (* Wake-up a thread waiting on an notification. *)
-definition
-  do_notification_transfer :: "cdl_object_id \<Rightarrow> unit k_monad"
-where
+definition do_notification_transfer :: "cdl_object_id \<Rightarrow> unit k_monad" where
   "do_notification_transfer receiver_id \<equiv> do
-      set_cap (receiver_id,tcb_pending_op_slot) RunningCap;
-      corrupt_tcb_intent receiver_id
+     set_cap (receiver_id,tcb_pending_op_slot) RunningCap;
+     corrupt_tcb_intent receiver_id
    od"
 
-(*
- * Signal on a notification.
- *
- * If someone is blocked on the notifications, we wake them up. Otherwise,
- * this is a no-(.)
- *)
-
-definition
-  send_signal_bound :: "cdl_object_id \<Rightarrow> unit k_monad"
-where
+(* Signal on a notification. If someone is blocked on the notifications, we wake them up.
+   Otherwise, this is a no-op.*)
+definition send_signal_bound :: "cdl_object_id \<Rightarrow> unit k_monad" where
   "send_signal_bound ntfn_id \<equiv> do
-      bound_tcbs \<leftarrow> gets $ get_waiting_sync_bound_ntfn_threads ntfn_id;
-      if (bound_tcbs \<noteq> {}) then do
-          t \<leftarrow> select bound_tcbs;
-          set_cap (t, tcb_pending_op_slot) NullCap;
-          do_notification_transfer t
-        od
-      else return ()
-    od"
-
-definition
-  send_signal :: "cdl_object_id \<Rightarrow> unit k_monad"
-where
-  "send_signal ep_id \<equiv>
-    (do waiters \<leftarrow> gets $ get_waiting_ntfn_recv_threads ep_id;
-          t \<leftarrow> option_select waiters;
-          case t of
-              None \<Rightarrow> return ()
-            | Some receiver \<Rightarrow> do_notification_transfer receiver
-     od)
-            \<sqinter> send_signal_bound ep_id"
-
-(*
- * Receive a signal (receive from a notification).
- *
- * We will either receive data or block waiting.
- *)
-definition
-  recv_signal :: "cdl_object_id \<Rightarrow> cdl_cap \<Rightarrow> unit k_monad"
-where
-  "recv_signal tcb_id_receiver ep_cap  \<equiv> do
-     ep_id \<leftarrow> return $ cap_object ep_cap;
-     block_thread_on_ipc tcb_id_receiver (PendingNtfnRecvCap ep_id) \<sqinter> corrupt_tcb_intent tcb_id_receiver
+     bound_tcbs \<leftarrow> gets $ get_waiting_sync_bound_ntfn_threads ntfn_id;
+     if bound_tcbs \<noteq> {} then do
+       t \<leftarrow> select bound_tcbs;
+       set_cap (t, tcb_pending_op_slot) NullCap;
+       do_notification_transfer t
+     od
+     else return ()
    od"
 
-(*
- * Send an IPC to the given endpoint. If someone is waiting, we wake
- * them up. Otherwise, we put the sender to sleep.
- *)
-definition
-  send_ipc :: "bool \<Rightarrow> bool \<Rightarrow> cdl_badge \<Rightarrow> bool \<Rightarrow> bool \<Rightarrow> cdl_object_id \<Rightarrow> cdl_object_id \<Rightarrow> unit k_monad"
-where
-  "send_ipc block call badge can_grant can_grant_reply tcb_id_sender ep_id \<equiv>
-    do
-      waiters \<leftarrow> gets $ get_waiting_sync_recv_threads ep_id;
-      t \<leftarrow> option_select waiters;
-      case t of
-          None \<Rightarrow>
-            if block then
-              block_thread_on_ipc tcb_id_sender
-                  (PendingSyncSendCap ep_id badge call can_grant can_grant_reply False)
-            else
-              return ()
-        | Some tcb_id_receiver \<Rightarrow> do
-             \<comment> \<open>liftM instead of bind+return avoids early unfolding in send_ipc_corres\<close>
-             recv_state \<leftarrow> liftM (\<lambda>tcb. the (cdl_tcb_caps tcb tcb_pending_op_slot)) $
-                              get_thread tcb_id_receiver;
-             reply_can_grant \<leftarrow>
-               (case recv_state of
-                    PendingSyncRecvCap target False receiver_grant \<Rightarrow> do
-                      do_ipc_transfer (Some ep_id) tcb_id_sender tcb_id_receiver can_grant;
-                      return receiver_grant od
-                  | _ \<Rightarrow> fail);
-             set_cap (tcb_id_receiver,tcb_pending_op_slot) RunningCap;
-             (when (can_grant \<or> can_grant_reply) $
-                  (inject_reply_cap tcb_id_sender tcb_id_receiver reply_can_grant))
-               \<sqinter> set_cap (tcb_id_sender,tcb_pending_op_slot) NullCap \<sqinter> return ()
-          od
-    od"
+definition send_signal :: "cdl_object_id \<Rightarrow> unit k_monad" where
+  "send_signal ep_id \<equiv>
+     do waiters \<leftarrow> gets $ get_waiting_ntfn_recv_threads ep_id;
+       t \<leftarrow> option_select waiters;
+       case t of
+         None \<Rightarrow> return ()
+       | Some receiver \<Rightarrow> do_notification_transfer receiver
+     od
+     \<sqinter> send_signal_bound ep_id"
 
-(*
- * Receive an IPC from the given endpoint. If someone is waiting, we
- * wake them up. Otherwise, we put the receiver to sleep.
- *)
-definition
-  receive_sync :: "cdl_object_id \<Rightarrow> cdl_object_id \<Rightarrow> bool \<Rightarrow> unit k_monad"
-where
-  "receive_sync thread ep_id receiver_can_grant \<equiv> do
-    waiters \<leftarrow> gets $ get_waiting_sync_send_threads ep_id;
-      waiter \<leftarrow> option_select waiters;
-      (case waiter of
-          None \<Rightarrow>
-            block_thread_on_ipc thread (PendingSyncRecvCap ep_id False receiver_can_grant)
-             \<sqinter> corrupt_tcb_intent thread
-        | Some tcb_id_sender \<Rightarrow> (do
-            tcb \<leftarrow> get_thread tcb_id_sender;
-            case ((cdl_tcb_caps tcb) tcb_pending_op_slot) of
-              Some (PendingSyncSendCap target _ call can_grant can_grant_reply fault) \<Rightarrow> (do
-                 do_ipc_transfer (Some ep_id) tcb_id_sender thread can_grant;
-                 (when (can_grant \<or> can_grant_reply) $
-                    (inject_reply_cap tcb_id_sender thread receiver_can_grant)) \<sqinter>
-                 set_cap (tcb_id_sender, tcb_pending_op_slot) RunningCap \<sqinter>
-                 set_cap (tcb_id_sender, tcb_pending_op_slot) NullCap
-              od)
-        od)
-      )
-    od"
+(* Receive a signal (receive from a notification).  We will either receive data or block waiting. *)
+definition recv_signal :: "cdl_object_id \<Rightarrow> cdl_cap \<Rightarrow> unit k_monad" where
+  "recv_signal tcb_id_receiver ep_cap \<equiv> do
+     ep_id \<leftarrow> return $ cap_object ep_cap;
+     block_thread_on_ipc tcb_id_receiver (PendingNtfnRecvCap ep_id)
+     \<sqinter> corrupt_tcb_intent tcb_id_receiver
+   od"
 
-(* This is more nonderministic than is really required, but
-   it makes the refinement proofs much easier *)
-definition
-  receive_ipc :: "cdl_object_id \<Rightarrow> cdl_object_id \<Rightarrow> bool \<Rightarrow> unit k_monad"
-where
-  "receive_ipc thread ep_id can_grant \<equiv> corrupt_tcb_intent thread \<sqinter> receive_sync thread ep_id can_grant"
-
-definition
-  invoke_endpoint :: "bool \<Rightarrow> bool \<Rightarrow> cdl_endpoint_invocation \<Rightarrow> unit k_monad"
-where
-  "invoke_endpoint is_call can_block params \<equiv> case params of
-    SyncMessage badge can_grant can_grant_reply ep_id \<Rightarrow> do
-      thread \<leftarrow> gets_the cdl_current_thread;
-      send_ipc can_block is_call badge can_grant can_grant_reply thread ep_id
-    od"
-
-definition
-  invoke_notification :: "cdl_notification_invocation \<Rightarrow> unit k_monad"
-where
-  "invoke_notification params \<equiv> case params of
-    Signal badge ep_id \<Rightarrow>
-      send_signal ep_id"
-
-definition
-  invoke_reply :: "cdl_reply_invocation \<Rightarrow> unit k_monad"
-where
-  "invoke_reply params \<equiv> case params of
-    ReplyMessage recv reply_cap_ref rights \<Rightarrow> do
-      send \<leftarrow> gets_the cdl_current_thread;
-      do_reply_transfer send recv reply_cap_ref rights
-    od"
-
-
-(*
- * Send a fault IPC to the given thread's fault handler.
- *)
-definition
-  send_fault_ipc :: "cdl_object_id \<Rightarrow> unit fault_monad"
+(* Send an IPC to the given endpoint. If someone is waiting, we wake  them up.
+   Otherwise, we put the sender to sleep. *)
+definition send_ipc ::
+  "bool \<Rightarrow> bool \<Rightarrow> cdl_badge \<Rightarrow> bool \<Rightarrow> bool \<Rightarrow> cdl_object_id \<Rightarrow> cdl_object_id \<Rightarrow> unit k_monad"
   where
-  "send_fault_ipc tcb_id \<equiv>
-    doE
-      \<comment> \<open>Lookup where we should send the fault IPC to.\<close>
-      tcb \<leftarrow> liftE $ get_thread tcb_id;
-      target_ep_cptr \<leftarrow> returnOk $ cdl_tcb_fault_endpoint tcb;
-      handler_cap \<leftarrow> lookup_cap tcb_id target_ep_cptr;
-      (case handler_cap of
-          EndpointCap ref badge rights \<Rightarrow>
-            if Write \<in> rights \<and> (Grant \<in> rights \<or> GrantReply \<in> rights) then
-              liftE $ do
-                update_thread_fault tcb_id (\<lambda>_. True);
-                send_ipc True True badge (Grant \<in> rights) True tcb_id ref
-              od
-            else
-               throw
-        | _ \<Rightarrow> throw)
-    odE"
+  "send_ipc block call badge can_grant can_grant_reply tcb_id_sender ep_id \<equiv> do
+     waiters \<leftarrow> gets $ get_waiting_sync_recv_threads ep_id;
+     t \<leftarrow> option_select waiters;
+     case t of
+       None \<Rightarrow> if block
+               then block_thread_on_ipc tcb_id_sender
+                                        (PendingSyncSendCap ep_id badge call can_grant
+                                                            can_grant_reply False)
+               else return ()
+     | Some tcb_id_receiver \<Rightarrow> do
+         \<comment> \<open>liftM instead of bind+return avoids early unfolding in send_ipc_corres\<close>
+         recv_state \<leftarrow> liftM (\<lambda>tcb. the (cdl_tcb_caps tcb tcb_pending_op_slot)) $
+                             get_thread tcb_id_receiver;
+         reply_can_grant \<leftarrow> case recv_state of
+                              PendingSyncRecvCap target False receiver_grant \<Rightarrow> do
+                                do_ipc_transfer (Some ep_id) tcb_id_sender tcb_id_receiver can_grant;
+                                return receiver_grant od
+                            | _ \<Rightarrow> fail;
+         set_cap (tcb_id_receiver,tcb_pending_op_slot) RunningCap;
+         when (can_grant \<or> can_grant_reply)
+              (inject_reply_cap tcb_id_sender tcb_id_receiver reply_can_grant)
+         \<sqinter> set_cap (tcb_id_sender,tcb_pending_op_slot) NullCap \<sqinter> return ()
+       od
+   od"
 
-(*
- * Handle a fault caused by the current thread.
- *
- * The abstract spec adds two additional parameters:
- *
- *    1. The fault type (which we abstract away);
- *
- *    2. The thread causing the fault (which always turns out
- *       to be the current thread).
- *)
-definition
-  handle_fault :: "unit k_monad"
-where
+(* Receive an IPC from the given endpoint. If someone is waiting, we wake them up. Otherwise, we
+   put the receiver to sleep. *)
+definition receive_sync :: "cdl_object_id \<Rightarrow> cdl_object_id \<Rightarrow> bool \<Rightarrow> unit k_monad" where
+  "receive_sync thread ep_id receiver_can_grant \<equiv> do
+     waiters \<leftarrow> gets $ get_waiting_sync_send_threads ep_id;
+     waiter \<leftarrow> option_select waiters;
+     case waiter of
+       None \<Rightarrow> block_thread_on_ipc thread (PendingSyncRecvCap ep_id False receiver_can_grant)
+               \<sqinter> corrupt_tcb_intent thread
+     | Some tcb_id_sender \<Rightarrow> do
+         tcb \<leftarrow> get_thread tcb_id_sender;
+         case cdl_tcb_caps tcb tcb_pending_op_slot of
+           Some (PendingSyncSendCap target _ call can_grant can_grant_reply fault) \<Rightarrow> do
+             do_ipc_transfer (Some ep_id) tcb_id_sender thread can_grant;
+             when (can_grant \<or> can_grant_reply)
+                  (inject_reply_cap tcb_id_sender thread receiver_can_grant)
+             \<sqinter> set_cap (tcb_id_sender, tcb_pending_op_slot) RunningCap
+             \<sqinter> set_cap (tcb_id_sender, tcb_pending_op_slot) NullCap
+           od
+       od
+   od"
+
+(* This is more nonderministic than is really required, but it makes the refinement proofs much easier *)
+definition receive_ipc :: "cdl_object_id \<Rightarrow> cdl_object_id \<Rightarrow> bool \<Rightarrow> unit k_monad" where
+  "receive_ipc thread ep_id can_grant \<equiv>
+     corrupt_tcb_intent thread \<sqinter> receive_sync thread ep_id can_grant"
+
+definition invoke_endpoint :: "bool \<Rightarrow> bool \<Rightarrow> cdl_endpoint_invocation \<Rightarrow> unit k_monad" where
+  "invoke_endpoint is_call can_block params \<equiv>
+     case params of
+       SyncMessage badge can_grant can_grant_reply ep_id \<Rightarrow> do
+         thread \<leftarrow> gets_the cdl_current_thread;
+         send_ipc can_block is_call badge can_grant can_grant_reply thread ep_id
+       od"
+
+definition invoke_notification :: "cdl_notification_invocation \<Rightarrow> unit k_monad" where
+  "invoke_notification params \<equiv> case params of Signal badge ep_id \<Rightarrow> send_signal ep_id"
+
+definition invoke_reply :: "cdl_reply_invocation \<Rightarrow> unit k_monad" where
+  "invoke_reply params \<equiv>
+     case params of
+       ReplyMessage recv reply_cap_ref rights \<Rightarrow> do
+         send \<leftarrow> gets_the cdl_current_thread;
+         do_reply_transfer send recv reply_cap_ref rights
+       od"
+
+(* Send a fault IPC to the given thread's fault handler. *)
+definition send_fault_ipc :: "cdl_object_id \<Rightarrow> unit fault_monad" where
+  "send_fault_ipc tcb_id \<equiv> doE
+     \<comment> \<open>Look up where we should send the fault IPC to.\<close>
+     tcb \<leftarrow> liftE $ get_thread tcb_id;
+     target_ep_cptr \<leftarrow> returnOk $ cdl_tcb_fault_endpoint tcb;
+     handler_cap \<leftarrow> lookup_cap tcb_id target_ep_cptr;
+     case handler_cap of
+       EndpointCap ref badge rights \<Rightarrow> if Write \<in> rights \<and> (Grant \<in> rights \<or> GrantReply \<in> rights)
+                                       then liftE $ do
+                                         update_thread_fault tcb_id (\<lambda>_. True);
+                                         send_ipc True True badge (Grant \<in> rights) True tcb_id ref
+                                       od
+                                       else throw
+     | _ \<Rightarrow> throw
+   odE"
+
+(* Handle a fault caused by the current thread.
+   The abstract spec adds two additional parameters:
+      1. The fault type (which we abstract away);
+      2. The thread causing the fault (which always turns out to be the current thread). *)
+definition handle_fault :: "unit k_monad" where
   "handle_fault \<equiv> do
-    tcb_id \<leftarrow> gets_the cdl_current_thread;
-    (send_fault_ipc tcb_id
-      <catch> (\<lambda>_. KHeap_D.set_cap (tcb_id,tcb_pending_op_slot) cdl_cap.NullCap))
-  od"
+     tcb_id \<leftarrow> gets_the cdl_current_thread;
+     send_fault_ipc tcb_id <catch> (\<lambda>_. set_cap (tcb_id, tcb_pending_op_slot) NullCap)
+   od"
 
 end
