spec/capDL/PageTableUnmap_D.thy
@@ -9,233 +9,189 @@
    architectures do not model unmapping. *)
 
 theory PageTableUnmap_D
-imports
-  Invocations_D
-  KHeap_D
+  imports
+    Invocations_D
+    KHeap_D
 begin
 
 \<comment> \<open>Return all slots in the system containing a cap with the given property.\<close>
-definition
-  slots_with :: "(cdl_cap \<Rightarrow> bool) \<Rightarrow> cdl_state \<Rightarrow> cdl_cap_ref set"
-where
+definition slots_with :: "(cdl_cap \<Rightarrow> bool) \<Rightarrow> cdl_state \<Rightarrow> cdl_cap_ref set" where
   "slots_with P s \<equiv> {(obj, slot). \<exists>x c. cdl_objects s obj = Some x \<and>
                                         has_slots x \<and>
                                         object_slots x slot = Some c \<and> P c}"
 
-
 \<comment> \<open>Remove a pending operation from the given TCB.\<close>
-definition
-  remove_pending_operation :: "cdl_tcb \<Rightarrow> cdl_cap \<Rightarrow> cdl_tcb"
-where
+definition remove_pending_operation :: "cdl_tcb \<Rightarrow> cdl_cap \<Rightarrow> cdl_tcb" where
   "remove_pending_operation t cap \<equiv> t\<lparr>cdl_tcb_caps := (cdl_tcb_caps t)(tcb_pending_op_slot \<mapsto> cap)\<rparr>"
 
-
 \<comment> \<open>Is the given thread pending on the given endpoint?\<close>
-definition
-  is_thread_blocked_on_endpoint :: "cdl_tcb \<Rightarrow> cdl_object_id \<Rightarrow> bool"
-where
+definition is_thread_blocked_on_endpoint :: "cdl_tcb \<Rightarrow> cdl_object_id \<Rightarrow> bool" where
   "is_thread_blocked_on_endpoint t ep \<equiv>
-    case (cdl_tcb_caps t tcb_pending_op_slot) of
-        Some (PendingSyncSendCap p _ _ _ _ _) \<Rightarrow> p = ep
-      | Some (PendingSyncRecvCap p is_reply _) \<Rightarrow> p = ep \<and> \<not> is_reply
-      | Some (PendingNtfnRecvCap p) \<Rightarrow> p = ep
-      | _ \<Rightarrow> False"
-
+     case cdl_tcb_caps t tcb_pending_op_slot of
+       Some (PendingSyncSendCap p _ _ _ _ _) \<Rightarrow> p = ep
+     | Some (PendingSyncRecvCap p is_reply _) \<Rightarrow> p = ep \<and> \<not> is_reply
+     | Some (PendingNtfnRecvCap p) \<Rightarrow> p = ep
+     | _ \<Rightarrow> False"
 
 \<comment> \<open>Cancel all pending IPCs currently blocked on this endpoint.\<close>
-definition
-  cancel_all_ipc :: "cdl_object_id \<Rightarrow> unit k_monad"
-where
+definition cancel_all_ipc :: "cdl_object_id \<Rightarrow> unit k_monad" where
   "cancel_all_ipc ep \<equiv>
-    modify (\<lambda>s. s\<lparr>cdl_objects :=  map_option
-        (\<lambda>obj. case obj of
-            Tcb t \<Rightarrow>
-              if (is_thread_blocked_on_endpoint t ep) then
-                Tcb (remove_pending_operation t RestartCap)
-              else
-                Tcb t
-           | _ \<Rightarrow> obj)
-          \<circ> (cdl_objects s)\<rparr>)"
+     modify (\<lambda>s. s\<lparr>cdl_objects :=
+                     map_option (\<lambda>obj. case obj of
+                                         Tcb t \<Rightarrow> if is_thread_blocked_on_endpoint t ep
+                                                  then Tcb (remove_pending_operation t RestartCap)
+                                                  else Tcb t
+                                       | _ \<Rightarrow> obj)
+                     \<circ> cdl_objects s\<rparr>)"
 
 \<comment> \<open>Is the given thread bound to the given ntfn?\<close>
-definition
-  is_thread_bound_to_ntfn :: "cdl_tcb \<Rightarrow> cdl_object_id \<Rightarrow> bool"
-where
+definition is_thread_bound_to_ntfn :: "cdl_tcb \<Rightarrow> cdl_object_id \<Rightarrow> bool" where
   "is_thread_bound_to_ntfn t ntfn \<equiv>
-    case (cdl_tcb_caps t tcb_boundntfn_slot) of
-        Some (BoundNotificationCap a) \<Rightarrow> a = ntfn
-      | _ \<Rightarrow> False"
+     case cdl_tcb_caps t tcb_boundntfn_slot of
+       Some (BoundNotificationCap a) \<Rightarrow> a = ntfn
+     | _ \<Rightarrow> False"
 
 \<comment> \<open>find all tcbs that are bound to a given ntfn\<close>
-definition
-  get_bound_notification_threads :: "cdl_object_id \<Rightarrow> cdl_state \<Rightarrow> cdl_object_id set"
-where
+definition get_bound_notification_threads :: "cdl_object_id \<Rightarrow> cdl_state \<Rightarrow> cdl_object_id set" where
   "get_bound_notification_threads ntfn_id state \<equiv>
-     {x. \<exists>a. (cdl_objects state) x = Some (Tcb a) \<and>
-         (((cdl_tcb_caps a) tcb_boundntfn_slot) = Some (BoundNotificationCap ntfn_id))}"
+     {t. \<exists>tcb. cdl_objects state t = Some (Tcb tcb) \<and>
+               cdl_tcb_caps tcb tcb_boundntfn_slot = Some (BoundNotificationCap ntfn_id)}"
 
-definition
-  modify_bound_ntfn :: "cdl_tcb \<Rightarrow> cdl_cap \<Rightarrow> cdl_tcb"
-where
-  "modify_bound_ntfn t cap \<equiv> t \<lparr> cdl_tcb_caps := (cdl_tcb_caps t)(tcb_boundntfn_slot \<mapsto> cap)\<rparr>"
+definition modify_bound_ntfn :: "cdl_tcb \<Rightarrow> cdl_cap \<Rightarrow> cdl_tcb" where
+  "modify_bound_ntfn t cap \<equiv> t \<lparr>cdl_tcb_caps := (cdl_tcb_caps t)(tcb_boundntfn_slot \<mapsto> cap)\<rparr>"
 
-
-abbreviation
-  do_unbind_notification :: "cdl_object_id \<Rightarrow> unit k_monad"
-where
+abbreviation do_unbind_notification :: "cdl_object_id \<Rightarrow> unit k_monad" where
   "do_unbind_notification tcb \<equiv> set_cap (tcb, tcb_boundntfn_slot) NullCap"
 
-definition
-  unbind_notification :: "cdl_object_id \<Rightarrow> unit k_monad"
-where
+definition unbind_notification :: "cdl_object_id \<Rightarrow> unit k_monad" where
   "unbind_notification tcb \<equiv> do
-     cap \<leftarrow> KHeap_D.get_cap (tcb, tcb_boundntfn_slot);
-     (case cap of
-      BoundNotificationCap _ \<Rightarrow> do_unbind_notification tcb
-    | _ \<Rightarrow> return ())
+     cap \<leftarrow> get_cap (tcb, tcb_boundntfn_slot);
+     case cap of
+       BoundNotificationCap _ \<Rightarrow> do_unbind_notification tcb
+     | _ \<Rightarrow> return ()
    od"
 
-definition
-  unbind_maybe_notification :: "cdl_object_id \<Rightarrow> unit k_monad"
-where
+definition unbind_maybe_notification :: "cdl_object_id \<Rightarrow> unit k_monad" where
   "unbind_maybe_notification ntfn_id \<equiv> do
      bound_tcbs \<leftarrow> gets $ get_bound_notification_threads ntfn_id;
      t \<leftarrow> option_select bound_tcbs;
-     (case t of
+     case t of
        None \<Rightarrow> return ()
-     | Some tcb \<Rightarrow> do_unbind_notification tcb)
-  od"
+     | Some tcb \<Rightarrow> do_unbind_notification tcb
+   od"
 
-definition
-  can_fast_finalise :: "cdl_cap \<Rightarrow> bool" where
- "can_fast_finalise cap \<equiv> case cap of ReplyCap r R \<Rightarrow> True
-                       | MasterReplyCap r \<Rightarrow> True
-                       | EndpointCap r b R \<Rightarrow> True
-                       | NotificationCap r b R \<Rightarrow> True
-                       | NullCap \<Rightarrow> True
-                       | RestartCap \<Rightarrow> True
-                       | RunningCap \<Rightarrow> True
-                       | PendingSyncSendCap r _ _ _ _ _ \<Rightarrow> True
-                       | PendingSyncRecvCap r _ _ \<Rightarrow> True
-                       | PendingNtfnRecvCap r \<Rightarrow> True
-                       | DomainCap \<Rightarrow> True
-                       | PageTableCap _ _ x _ \<Rightarrow> \<not>(x = Real)
-                       | FrameCap _ _ _ _ x _ \<Rightarrow> \<not>(x = Real)
-                       | _ \<Rightarrow> False"
+definition can_fast_finalise :: "cdl_cap \<Rightarrow> bool" where
+ "can_fast_finalise cap \<equiv>
+    case cap of
+      ReplyCap r R \<Rightarrow> True
+    | MasterReplyCap r \<Rightarrow> True
+    | EndpointCap r b R \<Rightarrow> True
+    | NotificationCap r b R \<Rightarrow> True
+    | NullCap \<Rightarrow> True
+    | RestartCap \<Rightarrow> True
+    | RunningCap \<Rightarrow> True
+    | PendingSyncSendCap r _ _ _ _ _ \<Rightarrow> True
+    | PendingSyncRecvCap r _ _ \<Rightarrow> True
+    | PendingNtfnRecvCap r \<Rightarrow> True
+    | DomainCap \<Rightarrow> True
+    | PageTableCap _ _ x _ \<Rightarrow> x \<noteq> Real
+    | FrameCap _ _ _ _ x _ \<Rightarrow> x \<noteq> Real
+    | _ \<Rightarrow> False"
 
 context
-notes [[function_internals =true]]
+  notes [[function_internals =true]]
 begin
 
-fun
-  fast_finalise :: "cdl_cap \<Rightarrow> bool \<Rightarrow> unit k_monad"
-where
-  "fast_finalise NullCap                  final = return ()"
-| "fast_finalise (RestartCap)             final = return ()"
-| "fast_finalise (RunningCap)             final = return ()"
-| "fast_finalise (ReplyCap r R)           final = return ()"
-| "fast_finalise (MasterReplyCap r)       final = return ()"
-| "fast_finalise (EndpointCap r b R)      final =
-      (when final $ cancel_all_ipc r)"
-| "fast_finalise (NotificationCap r b R) final =
-      (when final $ do
-            unbind_maybe_notification r;
-            cancel_all_ipc r
-          od)"
-| "fast_finalise (PendingSyncSendCap r _ _ _ _ _) final = return()"
-| "fast_finalise (PendingSyncRecvCap r _ _) final = return()"
-| "fast_finalise  (PendingNtfnRecvCap r) final = return()"
-| "fast_finalise DomainCap final = return ()"
-| "fast_finalise (PageTableCap _ _ x _) _ = (if x = Real then fail else return())"
-| "fast_finalise (FrameCap _ _ _ _ x _) _ = (if x = Real then fail else return())"
-| "fast_finalise _ _ = fail"
+fun fast_finalise :: "cdl_cap \<Rightarrow> bool \<Rightarrow> unit k_monad" where
+    "fast_finalise NullCap final = return ()"
+  | "fast_finalise RestartCap final = return ()"
+  | "fast_finalise RunningCap final = return ()"
+  | "fast_finalise (ReplyCap r R) final = return ()"
+  | "fast_finalise (MasterReplyCap r) final = return ()"
+  | "fast_finalise (EndpointCap r b R) final = when final (cancel_all_ipc r)"
+  | "fast_finalise (NotificationCap r b R) final =
+       (when final $ do
+          unbind_maybe_notification r;
+          cancel_all_ipc r
+        od)"
+  | "fast_finalise (PendingSyncSendCap r _ _ _ _ _) final = return()"
+  | "fast_finalise (PendingSyncRecvCap r _ _) final = return()"
+  | "fast_finalise  (PendingNtfnRecvCap r) final = return()"
+  | "fast_finalise DomainCap final = return ()"
+  | "fast_finalise (PageTableCap _ _ x _) _ = (if x = Real then fail else return())"
+  | "fast_finalise (FrameCap _ _ _ _ x _) _ = (if x = Real then fail else return())"
+  | "fast_finalise _ _ = fail"
 
 end
 
 \<comment> \<open>These caps don't count when determining if an entity should be deleted or not\<close>
-definition
-  cap_counts :: "cdl_cap \<Rightarrow> bool" where
- "cap_counts cap \<equiv> (case cap of
-    cdl_cap.NullCap \<Rightarrow> False
-  | UntypedCap _ _ _ \<Rightarrow> False
-  | ReplyCap _ _ \<Rightarrow> False
-  | MasterReplyCap _ \<Rightarrow> False
-  | RestartCap \<Rightarrow> False
-  | RunningCap \<Rightarrow> False
-  | PendingSyncSendCap _ _ _ _ _ _ \<Rightarrow> False
-  | PendingSyncRecvCap _ _ _ \<Rightarrow> False
-  | PendingNtfnRecvCap _ \<Rightarrow> False
-  | DomainCap \<Rightarrow> False
-  | BoundNotificationCap _ \<Rightarrow> False
-  | IrqControlCap  \<Rightarrow> False
-  | SGISignalCap _ _ \<Rightarrow> False
-  | AsidControlCap \<Rightarrow> False
-  | IOSpaceMasterCap \<Rightarrow> False
-  | FrameCap _ _ _ _ c _ \<Rightarrow> c = Real
-  | PageTableCap _ _ c _ \<Rightarrow> c = Real
-  | _ \<Rightarrow> True)"
+definition cap_counts :: "cdl_cap \<Rightarrow> bool" where
+  "cap_counts cap \<equiv> case cap of
+     cdl_cap.NullCap \<Rightarrow> False
+   | UntypedCap _ _ _ \<Rightarrow> False
+   | ReplyCap _ _ \<Rightarrow> False
+   | MasterReplyCap _ \<Rightarrow> False
+   | RestartCap \<Rightarrow> False
+   | RunningCap \<Rightarrow> False
+   | PendingSyncSendCap _ _ _ _ _ _ \<Rightarrow> False
+   | PendingSyncRecvCap _ _ _ \<Rightarrow> False
+   | PendingNtfnRecvCap _ \<Rightarrow> False
+   | DomainCap \<Rightarrow> False
+   | BoundNotificationCap _ \<Rightarrow> False
+   | IrqControlCap  \<Rightarrow> False
+   | SGISignalCap _ _ \<Rightarrow> False
+   | AsidControlCap \<Rightarrow> False
+   | IOSpaceMasterCap \<Rightarrow> False
+   | FrameCap _ _ _ _ c _ \<Rightarrow> c = Real
+   | PageTableCap _ _ c _ \<Rightarrow> c = Real
+   | _ \<Rightarrow> True"
 
-definition
-  cdl_cap_irq :: "cdl_cap \<Rightarrow> cdl_irq option" where
- "cdl_cap_irq cap \<equiv> (case cap of IrqHandlerCap irq \<Rightarrow> Some irq | _ \<Rightarrow> None)"
+definition cdl_cap_irq :: "cdl_cap \<Rightarrow> cdl_irq option" where
+  "cdl_cap_irq cap \<equiv> case cap of IrqHandlerCap irq \<Rightarrow> Some irq | _ \<Rightarrow> None"
 
 \<comment> \<open>Some caps don't count when determining if an entity should be deleted or not\<close>
-definition
-  is_final_cap' :: "cdl_cap \<Rightarrow> cdl_state \<Rightarrow> bool" where
- "is_final_cap' cap s \<equiv> ((cap_counts cap) \<and>
-  (\<exists>cref. {cref. \<exists>cap'. opt_cap cref s = Some cap'
-                       \<and> (cap_object cap = cap_object cap'
-                             \<and> cdl_cap_irq cap = cdl_cap_irq cap')
-                       \<and> cap_counts cap'}
-         = {cref}))"
+definition is_final_cap' :: "cdl_cap \<Rightarrow> cdl_state \<Rightarrow> bool" where
+  "is_final_cap' cap s \<equiv>
+     cap_counts cap \<and>
+     (\<exists>cref. {cref. \<exists>cap'. opt_cap cref s = Some cap' \<and>
+                           (cap_object cap = cap_object cap' \<and> cdl_cap_irq cap = cdl_cap_irq cap') \<and>
+                           cap_counts cap'} = {cref})"
 
-
-definition
-  is_final_cap :: "cdl_cap \<Rightarrow> bool k_monad" where
+definition is_final_cap :: "cdl_cap \<Rightarrow> bool k_monad" where
   "is_final_cap cap \<equiv> gets (is_final_cap' cap)"
 
+definition always_empty_slot :: "cdl_cap_ref \<Rightarrow> unit k_monad" where
+  "always_empty_slot slot = do
+     remove_parent slot;
+     set_cap slot NullCap
+   od"
 
-definition
-  always_empty_slot :: "cdl_cap_ref \<Rightarrow> unit k_monad"
-where
- "always_empty_slot slot = do
-    remove_parent slot;
-    set_cap slot NullCap
-  od"
-
-definition
-  empty_slot :: "cdl_cap_ref \<Rightarrow> unit k_monad"
-where
- "empty_slot slot = do
-  cap \<leftarrow> get_cap slot;
-  if cap = NullCap then
-    return ()
-  else do
-    remove_parent slot;
-    set_cap slot NullCap
-    od
-  od"
-
+definition empty_slot :: "cdl_cap_ref \<Rightarrow> unit k_monad"  where
+  "empty_slot slot = do
+     cap \<leftarrow> get_cap slot;
+     if cap = NullCap
+     then return ()
+     else do
+       remove_parent slot;
+       set_cap slot NullCap
+     od
+   od"
 
 text \<open>
- Non-premptable delete.
+  Non-premptable delete.
 
- Should only be used on deletes guaranteed not to preempt
- (and you are happy to prove this). In particular, it is
- useful for deleting caps that exist at the CapDL level
- but not at lower levels.
-\<close>
-definition
-  delete_cap_simple :: "cdl_cap_ref \<Rightarrow> unit k_monad"
-where
+  Should only be used on deletes guaranteed not to preempt (and you are happy to prove this).
+  In particular, it is useful for deleting caps that exist at the CapDL level  but not at lower
+  levels.\<close>
+definition delete_cap_simple :: "cdl_cap_ref \<Rightarrow> unit k_monad" where
   "delete_cap_simple cap_ref \<equiv> do
-    cap \<leftarrow> get_cap cap_ref;
-    unless (cap = NullCap) $ do
-      final \<leftarrow> is_final_cap cap;
-      fast_finalise cap final;
-      always_empty_slot cap_ref
-    od
-  od"
+     cap \<leftarrow> get_cap cap_ref;
+     unless (cap = NullCap) $ do
+       final \<leftarrow> is_final_cap cap;
+       fast_finalise cap final;
+       always_empty_slot cap_ref
+     od
+   od"
 
 
 text \<open>
@@ -244,127 +200,110 @@ text \<open>
   Should only be used on bounded revokes.
    * PageTableUnmap pt_cap_ref
    * PageUnmap frame_cap_ref \<Rightarrow>
-   * revoke_cap_simple (target_tcb, tcb_replycap_slot)
-\<close>
-function
-  revoke_cap_simple :: "cdl_cap_ref \<Rightarrow> unit k_monad"
-where
+   * revoke_cap_simple (target_tcb, tcb_replycap_slot)\<close>
+function revoke_cap_simple :: "cdl_cap_ref \<Rightarrow> unit k_monad" where
   "revoke_cap_simple victim s = (do
-    descendants \<leftarrow> gets $ KHeap_D.descendants_of victim;
-    assert (finite descendants);
-    non_null \<leftarrow> gets (\<lambda>s. {slot. opt_cap slot s \<noteq> Some NullCap \<and> opt_cap slot s \<noteq> None});
-    non_null_descendants \<leftarrow> return (descendants \<inter> non_null);
-    if (non_null_descendants \<noteq> {}) then do
-      a \<leftarrow> select non_null_descendants;
-      delete_cap_simple a;
-      revoke_cap_simple victim
-    od else return ()
-  od) s"
+     descendants \<leftarrow> gets $ descendants_of victim;
+     assert (finite descendants);
+     non_null \<leftarrow> gets (\<lambda>s. {slot. opt_cap slot s \<noteq> Some NullCap \<and> opt_cap slot s \<noteq> None});
+     non_null_descendants \<leftarrow> return (descendants \<inter> non_null);
+     if non_null_descendants \<noteq> {} then do
+       a \<leftarrow> select non_null_descendants;
+       delete_cap_simple a;
+       revoke_cap_simple victim
+     od else return ()
+   od) s"
   by auto
 
-definition cdl_get_pde :: "cdl_cap_ref \<Rightarrow> cdl_cap k_monad"
-where "cdl_get_pde ptr \<equiv>
-  KHeap_D.get_cap ptr"
+definition cdl_get_pde :: "cdl_cap_ref \<Rightarrow> cdl_cap k_monad" where
+  "cdl_get_pde ptr \<equiv> get_cap ptr"
 
-definition cdl_lookup_pd_slot :: "cdl_object_id \<Rightarrow> vptr \<Rightarrow> cdl_cap_ref"
-  where "cdl_lookup_pd_slot pd vptr \<equiv> (pd, unat (vptr >> sectionBits))"
+definition cdl_lookup_pd_slot :: "cdl_object_id \<Rightarrow> vptr \<Rightarrow> cdl_cap_ref" where
+  "cdl_lookup_pd_slot pd vptr \<equiv> (pd, unat (vptr >> sectionBits))"
 
-definition cdl_lookup_pt_slot :: "cdl_object_id \<Rightarrow> vptr \<Rightarrow> cdl_cap_ref except_monad"
-  where "cdl_lookup_pt_slot pd vptr \<equiv>
-    doE pd_slot \<leftarrow> returnOk (cdl_lookup_pd_slot pd vptr);
-        pdcap \<leftarrow> liftE $ cdl_get_pde pd_slot;
-        (case pdcap of cdl_cap.PageTableCap PT ref (Fake _) None
-         \<Rightarrow> ( doE pt \<leftarrow> returnOk ref;
-              pt_index \<leftarrow> returnOk ((vptr >> 12) && pt_slot_vaddr_mask);
-              returnOk (pt,unat pt_index)
-         odE)
-        | _ \<Rightarrow> Monads_D.throw)
-    odE"
+definition cdl_lookup_pt_slot :: "cdl_object_id \<Rightarrow> vptr \<Rightarrow> cdl_cap_ref except_monad" where
+  "cdl_lookup_pt_slot pd vptr \<equiv> doE
+     pd_slot \<leftarrow> returnOk (cdl_lookup_pd_slot pd vptr);
+     pdcap \<leftarrow> liftE $ cdl_get_pde pd_slot;
+     case pdcap of cdl_cap.PageTableCap PT ref (Fake _)
+       None \<Rightarrow> doE pt \<leftarrow> returnOk ref;
+                   pt_index \<leftarrow> returnOk ((vptr >> 12) && pt_slot_vaddr_mask);
+                   returnOk (pt, unat pt_index)
+               odE
+     | _ \<Rightarrow> throw
+   odE"
 
-definition
-  cdl_find_pd_for_asid :: "cdl_mapped_addr \<Rightarrow> cdl_object_id except_monad"
-where
+definition cdl_find_pd_for_asid :: "cdl_mapped_addr \<Rightarrow> cdl_object_id except_monad" where
   "cdl_find_pd_for_asid maddr \<equiv> doE
      asid_table \<leftarrow> liftE $ gets cdl_asid_table;
      asid_pool \<leftarrow> returnOk $ asid_table (fst (fst maddr));
-     pd_cap_ref \<leftarrow>
-       case asid_pool of
-         Some (AsidPoolCap ptr _) \<Rightarrow> returnOk (ptr, (snd \<circ> fst) maddr)
-       | _ \<Rightarrow> throw;
+     pd_cap_ref \<leftarrow> case asid_pool of
+                     Some (AsidPoolCap ptr _) \<Rightarrow> returnOk (ptr, (snd \<circ> fst) maddr)
+                   | _ \<Rightarrow> throw;
      pd_cap \<leftarrow> liftE $ get_cap pd_cap_ref;
      case pd_cap of PageTableCap PD pd _ _ \<Rightarrow> returnOk pd | _ \<Rightarrow> throw
-   odE "
+   odE"
 
 definition cdl_page_mapping_entries ::
   "vptr \<Rightarrow> nat \<Rightarrow> cdl_object_id \<Rightarrow> cdl_cap_ref except_monad"
   where
   "cdl_page_mapping_entries vptr pgsz pd \<equiv>
-   if pgsz = 12 then doE
-     p \<leftarrow> cdl_lookup_pt_slot pd vptr;
-          returnOk p
-   odE
-   else if pgsz = 16 then doE
-     p \<leftarrow> cdl_lookup_pt_slot pd vptr;
-          returnOk p
+     if pgsz = 12 then doE
+       p \<leftarrow> cdl_lookup_pt_slot pd vptr;
+            returnOk p
      odE
-   else if pgsz = sectionBits then doE
-     p \<leftarrow> returnOk $ cdl_lookup_pd_slot pd vptr;
-          returnOk p
-   odE
-   else if pgsz = superSectionBits then doE
-     p \<leftarrow> returnOk $ cdl_lookup_pd_slot pd vptr;
-          returnOk p
-   odE
-   else throw"
+     else if pgsz = 16 then doE
+       p \<leftarrow> cdl_lookup_pt_slot pd vptr;
+            returnOk p
+       odE
+     else if pgsz = sectionBits then doE
+       p \<leftarrow> returnOk $ cdl_lookup_pd_slot pd vptr;
+            returnOk p
+     odE
+     else if pgsz = superSectionBits then doE
+       p \<leftarrow> returnOk $ cdl_lookup_pd_slot pd vptr;
+            returnOk p
+     odE
+     else throw"
 
-definition
-  cdl_page_table_mapped :: "cdl_mapped_addr \<Rightarrow> cdl_object_id \<Rightarrow> (cdl_cap_ref option) k_monad"
-where
+definition cdl_page_table_mapped ::
+  "cdl_mapped_addr \<Rightarrow> cdl_object_id \<Rightarrow> (cdl_cap_ref option) k_monad" where
   "cdl_page_table_mapped maddr pt_id \<equiv> doE
      pd \<leftarrow> cdl_find_pd_for_asid maddr;
      pd_slot \<leftarrow> returnOk (cdl_lookup_pd_slot pd (snd maddr));
      pdcap \<leftarrow> liftE $ cdl_get_pde pd_slot;
-     (case pdcap of
-       cdl_cap.PageTableCap PT ref (Fake _) None \<Rightarrow>
-         (returnOk $ if ref = pt_id then Some pd_slot else None)
-     | _ \<Rightarrow> returnOk None )
-   odE <catch> (K (return None))"
+     case pdcap of
+       PageTableCap PT ref (Fake _) None \<Rightarrow> returnOk $ if ref = pt_id then Some pd_slot else None
+     | _ \<Rightarrow> returnOk None
+   odE <catch> K (return None)"
 
-text \<open>
-  Unmap a frame.
-\<close>
 
-definition
- "might_throw \<equiv> returnOk () \<sqinter> throw"
+text \<open>Unmap a frame.\<close>
 
-definition
-  unmap_page :: "cdl_mapped_addr  \<Rightarrow> cdl_object_id \<Rightarrow> nat \<Rightarrow> unit k_monad"
-where
-  "unmap_page maddr frame_id pgsz \<equiv>
-    doE
-      pd \<leftarrow> cdl_find_pd_for_asid maddr;
-      pslot \<leftarrow> cdl_page_mapping_entries (snd maddr) pgsz pd;
-      might_throw;
-      liftE $ delete_cap_simple pslot;
-      returnOk ()
-    odE <catch> (K $ return ())"
+definition might_throw :: "('a + unit) k_monad" where
+   "might_throw \<equiv> returnOk () \<sqinter> throw"
+
+definition unmap_page :: "cdl_mapped_addr  \<Rightarrow> cdl_object_id \<Rightarrow> nat \<Rightarrow> unit k_monad" where
+  "unmap_page maddr frame_id pgsz \<equiv> doE
+     pd \<leftarrow> cdl_find_pd_for_asid maddr;
+     pslot \<leftarrow> cdl_page_mapping_entries (snd maddr) pgsz pd;
+     might_throw;
+     liftE $ delete_cap_simple pslot;
+     returnOk ()
+   odE <catch> (K $ return ())"
 
 
 text \<open>
   Unmap a page table.
 
-  This hits the same problems as 'unmap_page', so we also
-  non-deterministically choose a bunch of page-tables to unmap.
-\<close>
-definition
-  unmap_page_table  :: "cdl_mapped_addr \<Rightarrow> cdl_object_id  \<Rightarrow> unit k_monad"
-where
-  "unmap_page_table maddr pt_id\<equiv>
-    do
-      pt_slot \<leftarrow> cdl_page_table_mapped maddr pt_id;
-      case pt_slot of (Some slot) \<Rightarrow> delete_cap_simple slot
-      | None \<Rightarrow> return ()
-    od"
-
+  This hits the same problems as 'unmap_page', so we also non-deterministically choose a bunch of
+  page-tables to unmap.\<close>
+definition unmap_page_table  :: "cdl_mapped_addr \<Rightarrow> cdl_object_id  \<Rightarrow> unit k_monad" where
+  "unmap_page_table maddr pt_id \<equiv> do
+     pt_slot \<leftarrow> cdl_page_table_mapped maddr pt_id;
+     case pt_slot of
+       Some slot \<Rightarrow> delete_cap_simple slot
+     | None \<Rightarrow> return ()
+   od"
 
 end
