spec/capDL/Schedule_D.thy
@@ -5,49 +5,35 @@
  *)
 
 theory Schedule_D
-imports KHeap_D
+  imports KHeap_D
 begin
 
-(*
- * Collect the set of runnable threads in the system.
- *)
-definition
-  all_active_tcbs :: "cdl_state \<Rightarrow> cdl_object_id set"
-where
-  "all_active_tcbs state \<equiv> {x \<in> dom (cdl_objects state).
-      \<exists> a. (cdl_objects state) x = Some (Tcb a)
-          \<and> ( ((cdl_tcb_caps a) tcb_pending_op_slot) = (Some RunningCap) \<or> ((cdl_tcb_caps a) tcb_pending_op_slot) = (Some RestartCap))}"
+(* Collect the set of runnable threads in the system. *)
+definition all_active_tcbs :: "cdl_state \<Rightarrow> cdl_object_id set" where
+  "all_active_tcbs state \<equiv>
+     {x \<in> dom (cdl_objects state). \<exists>a. cdl_objects state x = Some (Tcb a) \<and>
+                                       (cdl_tcb_caps a tcb_pending_op_slot = Some RunningCap \<or>
+                                        cdl_tcb_caps a tcb_pending_op_slot = Some RestartCap)}"
 
-definition
-  active_tcbs_in_domain :: "domain \<Rightarrow> cdl_state \<Rightarrow> cdl_object_id set"
-where
-  "active_tcbs_in_domain domain state  = {x \<in> dom (cdl_objects state).
-      \<exists> a. (cdl_objects state) x = Some (Tcb a)
-          \<and> ( ((cdl_tcb_caps a) tcb_pending_op_slot) = (Some RunningCap) \<or> ((cdl_tcb_caps a) tcb_pending_op_slot) = (Some RestartCap))
-          \<and> cdl_tcb_domain a = domain }"
+definition active_tcbs_in_domain :: "domain \<Rightarrow> cdl_state \<Rightarrow> cdl_object_id set" where
+  "active_tcbs_in_domain domain state \<equiv>
+     {x \<in> dom (cdl_objects state). \<exists>a. cdl_objects state x = Some (Tcb a) \<and>
+                                       (cdl_tcb_caps a tcb_pending_op_slot = Some RunningCap \<or>
+                                        cdl_tcb_caps a tcb_pending_op_slot = Some RestartCap) \<and>
+                                       cdl_tcb_domain a = domain }"
 
-(*
- * Switch to a new thread.
- *)
-definition
-  switch_to_thread :: "cdl_object_id option \<Rightarrow> unit k_monad"
-where
-  "switch_to_thread target \<equiv>
-     modify (\<lambda> t. t\<lparr> cdl_current_thread := target \<rparr>)"
+(* Switch to a new thread. *)
+definition switch_to_thread :: "cdl_object_id option \<Rightarrow> unit k_monad" where
+  "switch_to_thread target \<equiv> modify (\<lambda> t. t\<lparr> cdl_current_thread := target \<rparr>)"
 
-definition
-  change_current_domain :: "unit k_monad"
-where
+definition change_current_domain :: "unit k_monad" where
   "change_current_domain = do
      next_domain \<leftarrow> select UNIV;
-     modify      (\<lambda>s. s\<lparr> cdl_current_domain := next_domain \<rparr>)
+     modify (\<lambda>s. s\<lparr> cdl_current_domain := next_domain \<rparr>)
    od"
-(*
- * Scheduling is fully nondeterministic at this level.
- *)
-definition
-  schedule :: "unit k_monad"
-where
+
+(* Scheduling is fully nondeterministic at this level. *)
+definition schedule :: "unit k_monad" where
   "schedule \<equiv> do
      change_current_domain;
      next_domain \<leftarrow> gets cdl_current_domain;
@@ -59,7 +45,4 @@ where
      switch_to_thread None
    od"
 
-
 end
-
-
