spec/capDL/Tcb_D.thy
@@ -4,305 +4,288 @@
  * SPDX-License-Identifier: GPL-2.0-only
  *)
 
-(*
- * Operations on thread control blocks.
- *)
+(* Operations on thread control blocks. *)
 
 theory Tcb_D
-imports Invocations_D CSpace_D ExecSpec.Structs_B
+  imports
+    Invocations_D
+    CSpace_D
+    ExecSpec.Structs_B
 begin
 
-definition cdl_update_cnode_cap_data :: "cdl_cap \<Rightarrow> machine_word \<Rightarrow> cdl_cap"
-where "cdl_update_cnode_cap_data cap data  \<equiv>
-  case cap of cdl_cap.CNodeCap oid _ _ sz \<Rightarrow> if data\<noteq>0 then
-    (let reserved_bits = 3; guard_bits = 18; guard_size_bits = 5; new_guard_size = unat ((data >> reserved_bits) && mask guard_size_bits);
-        new_guard =
-          (data >> reserved_bits + guard_size_bits) && mask (min (unat ((data >> reserved_bits) && mask guard_size_bits)) guard_bits)
-    in CNodeCap oid new_guard new_guard_size sz)
-    else cap
-  | _ \<Rightarrow> cap"
+definition cdl_update_cnode_cap_data :: "cdl_cap \<Rightarrow> machine_word \<Rightarrow> cdl_cap" where
+  "cdl_update_cnode_cap_data cap data  \<equiv>
+     case cap of CNodeCap oid _ _ sz \<Rightarrow>
+       if data \<noteq> 0 then
+         let
+           reserved_bits = 3; \<comment> \<open>FIXME: magic numbers\<close>
+           guard_bits = 18;
+           guard_size_bits = 5;
+           new_guard_size = unat ((data >> reserved_bits) && mask guard_size_bits);
+           new_guard = (data >> reserved_bits + guard_size_bits) &&
+                       mask (min (unat ((data >> reserved_bits) && mask guard_size_bits)) guard_bits)
+         in
+           CNodeCap oid new_guard new_guard_size sz
+       else cap
+     | _ \<Rightarrow> cap"
 
-definition cdl_same_arch_obj_as :: "cdl_cap \<Rightarrow> cdl_cap \<Rightarrow> bool"
-where "cdl_same_arch_obj_as capa capb \<equiv>
-  case capa of AsidPoolCap x _ \<Rightarrow> (
-        case capb of AsidPoolCap y _ \<Rightarrow>  y = x
-        | _ \<Rightarrow> False)
-  | AsidControlCap \<Rightarrow> (
-       case capb of AsidControlCap \<Rightarrow> True
-        | _ \<Rightarrow> False)
-  | FrameCap dev ra _ sa _ _ \<Rightarrow> (
-       case capb of FrameCap dev' rb _ sb _ _ \<Rightarrow> rb = ra \<and> sb = sa \<and> dev = dev'
-        | _ \<Rightarrow> False)
-  | cdl_cap.PageTableCap l a _ _ \<Rightarrow> (
-       case capb of cdl_cap.PageTableCap l' b _ _ \<Rightarrow> b = a \<and> l' = l
-        | _ \<Rightarrow> False)
-  | _ \<Rightarrow> False"
+definition cdl_same_arch_obj_as :: "cdl_cap \<Rightarrow> cdl_cap \<Rightarrow> bool" where
+  "cdl_same_arch_obj_as capa capb \<equiv>
+     case capa of
+       AsidPoolCap x _ \<Rightarrow> (case capb of AsidPoolCap y _ \<Rightarrow> y = x | _ \<Rightarrow> False)
+     | AsidControlCap \<Rightarrow> (case capb of AsidControlCap \<Rightarrow> True | _ \<Rightarrow> False)
+     | FrameCap dev ra _ sa _ _ \<Rightarrow>
+         (case capb of FrameCap dev' rb _ sb _ _ \<Rightarrow> rb = ra \<and> sb = sa \<and> dev = dev' | _ \<Rightarrow> False)
+     | PageTableCap l a _ _ \<Rightarrow>
+         (case capb of PageTableCap l' b _ _ \<Rightarrow> b = a \<and> l' = l | _ \<Rightarrow> False)
+     | _ \<Rightarrow> False"
 
-definition
-  decode_tcb_invocation :: "cdl_cap \<Rightarrow> cdl_cap_ref \<Rightarrow> (cdl_cap \<times> cdl_cap_ref) list \<Rightarrow>
-      cdl_tcb_intent \<Rightarrow> cdl_tcb_invocation except_monad"
-where
-  "decode_tcb_invocation target slot caps intent \<equiv> case intent of
-       \<comment> \<open>Read another thread's registers.\<close>
-       TcbReadRegistersIntent suspend flags count \<Rightarrow>
-         returnOk (ReadRegisters (cap_object target) suspend 0 0) \<sqinter> throw
+definition decode_tcb_invocation ::
+  "cdl_cap \<Rightarrow> cdl_cap_ref \<Rightarrow> (cdl_cap \<times> cdl_cap_ref) list \<Rightarrow> cdl_tcb_intent \<Rightarrow>
+   cdl_tcb_invocation except_monad" where
+  "decode_tcb_invocation target slot caps intent \<equiv>
+     case intent of
+        \<comment> \<open>Read another thread's registers.\<close>
+        TcbReadRegistersIntent suspend flags count \<Rightarrow>
+          returnOk (ReadRegisters (cap_object target) suspend 0 0) \<sqinter> throw
 
-       \<comment> \<open>Write another thread's registers.\<close>
-     | TcbWriteRegistersIntent resume flags count regs \<Rightarrow>
-         returnOk (WriteRegisters (cap_object target) resume [0] 0) \<sqinter> throw
+        \<comment> \<open>Write another thread's registers.\<close>
+      | TcbWriteRegistersIntent resume flags count regs \<Rightarrow>
+          returnOk (WriteRegisters (cap_object target) resume [0] 0) \<sqinter> throw
 
-       \<comment> \<open>Copy registers from one thread to another.\<close>
-     | TcbCopyRegistersIntent suspend_source resume_target f1 f2 f3 \<Rightarrow>
-         doE
-           (source_cap, _) \<leftarrow> throw_on_none $ get_index caps 0;
-           source_tcb \<leftarrow> (
-              case source_cap of
-                  TcbCap x \<Rightarrow> returnOk x
-                | _ \<Rightarrow> throw);
-           target_tcb \<leftarrow> returnOk $ cap_object target;
-           returnOk (CopyRegisters target_tcb source_tcb suspend_source resume_target f1 f2 0)
-         odE \<sqinter> throw
-
-       \<comment> \<open>Suspend the target thread.\<close>
-     | TcbSuspendIntent \<Rightarrow>
-         returnOk (Suspend (cap_object target)) \<sqinter> throw
-
-       \<comment> \<open>Resume the target thread.\<close>
-     | TcbResumeIntent \<Rightarrow>
-         returnOk (Resume (cap_object target)) \<sqinter> throw
-
-       \<comment> \<open>Configure: target, fault_ep, mcp, priority, cspace_root_data, vspace_root_data, buffer\<close>
-     | TcbConfigureIntent fault_ep cspace_root_data vspace_root_data buffer \<Rightarrow>
-         doE
-           cspace_root \<leftarrow> throw_on_none $ get_index caps 0;
-           vspace_root \<leftarrow> throw_on_none $ get_index caps 1;
-           buffer_frame \<leftarrow> throw_on_none $ get_index caps 2;
-           cspace_root_cap_ref \<leftarrow> returnOk $ (cdl_update_cnode_cap_data (fst cspace_root) cspace_root_data,snd cspace_root);
-           vspace_root_cap_ref \<leftarrow> returnOk $ vspace_root;
-           buffer_frame_opt \<leftarrow> returnOk $ (if (buffer \<noteq> 0) then Some (reset_mem_mapping (fst buffer_frame), snd buffer_frame) else None);
-           returnOk (ThreadControl (cap_object target) slot (Some fault_ep)
-               (Some cspace_root_cap_ref) (Some vspace_root_cap_ref) (buffer_frame_opt))
-         odE \<sqinter> throw
-
-       \<comment> \<open>Modify a thread's maximum control priority.\<close>
-     | TcbSetMCPriorityIntent mcp \<Rightarrow>
-         doE
-           auth_cap \<leftarrow> throw_on_none $ get_index caps 0;
-           returnOk (ThreadControl (cap_object target) slot None None None None)
-         odE \<sqinter> throw
-
-       \<comment> \<open>Modify a thread's priority.\<close>
-     | TcbSetPriorityIntent priority \<Rightarrow>
-         doE
-           auth_cap \<leftarrow> throw_on_none $ get_index caps 0;
-           returnOk (ThreadControl (cap_object target) slot None None None None)
-         odE \<sqinter> throw
-
-       \<comment> \<open>Modify a thread's mcp and priority at the same time.\<close>
-     | TcbSetSchedParamsIntent mcp priority \<Rightarrow>
-         doE
-           auth_cap \<leftarrow> throw_on_none $ get_index caps 0;
-           returnOk (ThreadControl (cap_object target) slot None None None None)
-         odE \<sqinter> throw
-
-       \<comment> \<open>Modify a thread's IPC buffer.\<close>
-     | TcbSetIPCBufferIntent buffer \<Rightarrow>
-         doE
-           buffer_frame \<leftarrow> throw_on_none $ get_index caps 0;
-           buffer_frame_opt \<leftarrow> returnOk $ (if (buffer \<noteq> 0) then Some (reset_mem_mapping (fst buffer_frame), snd buffer_frame) else None);
-           returnOk (ThreadControl (cap_object target) slot None None None buffer_frame_opt)
-         odE \<sqinter> throw
-
-       \<comment> \<open>Update the various spaces (CSpace/VSpace) of a thread.\<close>
-     | TcbSetSpaceIntent fault_ep cspace_root_data vspace_root_data \<Rightarrow>
-         doE
-           cspace_root \<leftarrow> throw_on_none $ get_index caps 0;
-           vspace_root \<leftarrow> throw_on_none $ get_index caps 1;
-           cspace_root_cap_ref \<leftarrow> returnOk $ (cdl_update_cnode_cap_data (fst cspace_root) cspace_root_data,snd cspace_root);
-           vspace_root_cap_ref \<leftarrow> returnOk $ vspace_root;
-           returnOk (ThreadControl (cap_object target) slot (Some fault_ep)
-               (Some cspace_root_cap_ref) (Some vspace_root_cap_ref) None)
+        \<comment> \<open>Copy registers from one thread to another.\<close>
+      | TcbCopyRegistersIntent suspend_source resume_target f1 f2 f3 \<Rightarrow> doE
+          (source_cap, _) \<leftarrow> throw_on_none $ get_index caps 0;
+          source_tcb \<leftarrow> case source_cap of TcbCap x \<Rightarrow> returnOk x | _ \<Rightarrow> throw;
+          target_tcb \<leftarrow> returnOk $ cap_object target;
+          returnOk (CopyRegisters target_tcb source_tcb suspend_source resume_target f1 f2 0)
         odE \<sqinter> throw
-     | TcbBindNTFNIntent \<Rightarrow> doE
-           (ntfn_cap, _) \<leftarrow> throw_on_none $ get_index caps 0;
-           returnOk (NotificationControl (cap_object target) (Some (cap_object ntfn_cap)))
+
+        \<comment> \<open>Suspend the target thread.\<close>
+      | TcbSuspendIntent \<Rightarrow>
+          returnOk (Suspend (cap_object target)) \<sqinter> throw
+
+        \<comment> \<open>Resume the target thread.\<close>
+      | TcbResumeIntent \<Rightarrow>
+          returnOk (Resume (cap_object target)) \<sqinter> throw
+
+        \<comment> \<open>Configure: target, fault_ep, mcp, priority, cspace_root_data, vspace_root_data, buffer\<close>
+      | TcbConfigureIntent fault_ep cspace_root_data vspace_root_data buffer \<Rightarrow> doE
+          cspace_root \<leftarrow> throw_on_none $ get_index caps 0;
+          vspace_root \<leftarrow> throw_on_none $ get_index caps 1;
+          buffer_frame \<leftarrow> throw_on_none $ get_index caps 2;
+          cspace_root_cap_ref \<leftarrow> returnOk (cdl_update_cnode_cap_data (fst cspace_root)
+                                                                     cspace_root_data,
+                                           snd cspace_root);
+          vspace_root_cap_ref \<leftarrow> returnOk $ vspace_root;
+          buffer_frame_opt \<leftarrow> returnOk (if buffer \<noteq> 0
+                                        then Some (reset_mem_mapping (fst buffer_frame),
+                                                   snd buffer_frame)
+                                        else None);
+          returnOk $ ThreadControl (cap_object target) slot (Some fault_ep)
+                                   (Some cspace_root_cap_ref) (Some vspace_root_cap_ref)
+                                   (buffer_frame_opt)
          odE \<sqinter> throw
-     | TcbUnbindNTFNIntent \<Rightarrow> returnOk (NotificationControl (cap_object target) None) \<sqinter> throw
-     | TcbSetTLSBaseIntent \<Rightarrow> returnOk (SetTLSBase (cap_object target)) \<sqinter> throw
-     | TcbSetFlagsIntent set_flags clear_flags \<Rightarrow>
-         returnOk (SetFlags (cap_object target) (set_flags && tcbFlagMask) (clear_flags && tcbFlagMask)) \<sqinter> throw"
+
+        \<comment> \<open>Modify a thread's maximum control priority.\<close>
+      | TcbSetMCPriorityIntent mcp \<Rightarrow> doE
+          auth_cap \<leftarrow> throw_on_none $ get_index caps 0;
+          returnOk $ ThreadControl (cap_object target) slot None None None None
+        odE \<sqinter> throw
+
+        \<comment> \<open>Modify a thread's priority.\<close>
+      | TcbSetPriorityIntent priority \<Rightarrow> doE
+          auth_cap \<leftarrow> throw_on_none $ get_index caps 0;
+          returnOk $ ThreadControl (cap_object target) slot None None None None
+        odE \<sqinter> throw
+
+        \<comment> \<open>Modify a thread's mcp and priority at the same time.\<close>
+      | TcbSetSchedParamsIntent mcp priority \<Rightarrow> doE
+          auth_cap \<leftarrow> throw_on_none $ get_index caps 0;
+          returnOk $ ThreadControl (cap_object target) slot None None None None
+        odE \<sqinter> throw
+
+        \<comment> \<open>Modify a thread's IPC buffer.\<close>
+      | TcbSetIPCBufferIntent buffer \<Rightarrow> doE
+          buffer_frame \<leftarrow> throw_on_none $ get_index caps 0;
+          buffer_frame_opt \<leftarrow> returnOk (if buffer \<noteq> 0
+                                        then Some (reset_mem_mapping (fst buffer_frame),
+                                                   snd buffer_frame)
+                                        else None);
+          returnOk (ThreadControl (cap_object target) slot None None None buffer_frame_opt)
+        odE \<sqinter> throw
+
+        \<comment> \<open>Update the various spaces (CSpace/VSpace) of a thread.\<close>
+      | TcbSetSpaceIntent fault_ep cspace_root_data vspace_root_data \<Rightarrow> doE
+          cspace_root \<leftarrow> throw_on_none $ get_index caps 0;
+          vspace_root \<leftarrow> throw_on_none $ get_index caps 1;
+          cspace_root_cap_ref \<leftarrow> returnOk (cdl_update_cnode_cap_data (fst cspace_root)
+                                                                     cspace_root_data,
+                                           snd cspace_root);
+          vspace_root_cap_ref \<leftarrow> returnOk $ vspace_root;
+          returnOk $ ThreadControl (cap_object target) slot (Some fault_ep)
+                                   (Some cspace_root_cap_ref) (Some vspace_root_cap_ref) None
+         odE \<sqinter> throw
+      | TcbBindNTFNIntent \<Rightarrow> doE
+          (ntfn_cap, _) \<leftarrow> throw_on_none $ get_index caps 0;
+          returnOk (NotificationControl (cap_object target) (Some (cap_object ntfn_cap)))
+        odE \<sqinter> throw
+      | TcbUnbindNTFNIntent \<Rightarrow> returnOk (NotificationControl (cap_object target) None) \<sqinter> throw
+      | TcbSetTLSBaseIntent \<Rightarrow> returnOk (SetTLSBase (cap_object target)) \<sqinter> throw
+      | TcbSetFlagsIntent set_flags clear_flags \<Rightarrow>
+          returnOk (SetFlags (cap_object target)
+                             (set_flags && tcbFlagMask)
+                             (clear_flags && tcbFlagMask))
+          \<sqinter> throw"
 
 
 (* Delete the given slot of a TCB. *)
-
-definition
-  tcb_empty_thread_slot :: "cdl_object_id \<Rightarrow> cdl_cnode_index \<Rightarrow> unit preempt_monad"
-where
+definition tcb_empty_thread_slot :: "cdl_object_id \<Rightarrow> cdl_cnode_index \<Rightarrow> unit preempt_monad" where
   "tcb_empty_thread_slot target_tcb target_slot \<equiv> doE
-    cap \<leftarrow> liftE $ get_cap (target_tcb,target_slot);
-    whenE (cap \<noteq> NullCap) $
-      delete_cap  (target_tcb, target_slot)
-  odE"
+     cap \<leftarrow> liftE $ get_cap (target_tcb,target_slot);
+     whenE (cap \<noteq> NullCap) $ delete_cap (target_tcb, target_slot)
+   odE"
 
-(* Update the given slot of a TCB with a new cap, delete the previous
- * capability that was in the slot. *)
-
-definition
-  tcb_update_thread_slot :: "cdl_object_id \<Rightarrow> cdl_cap_ref \<Rightarrow> cdl_cnode_index \<Rightarrow> (cdl_cap \<times> cdl_cap_ref) \<Rightarrow> unit preempt_monad"
-where
-  "tcb_update_thread_slot target_tcb tcb_cap_slot target_slot pcap \<equiv>
-         liftE (do
-           thread_cap \<leftarrow> get_cap tcb_cap_slot;
-           when (thread_cap = TcbCap target_tcb)
-           (insert_cap_child (fst pcap) (snd pcap) (target_tcb, target_slot)
-            \<sqinter> insert_cap_sibling (fst pcap) (snd pcap) (target_tcb,target_slot))
-         od)"
+(* Update the given slot of a TCB with a new cap, delete the previous capability in the slot. *)
+definition tcb_update_thread_slot ::
+  "cdl_object_id \<Rightarrow> cdl_cap_ref \<Rightarrow> cdl_cnode_index \<Rightarrow> (cdl_cap \<times> cdl_cap_ref) \<Rightarrow> unit preempt_monad"
+  where
+  "tcb_update_thread_slot target_tcb tcb_cap_slot target_slot pcap \<equiv> liftE (do
+     thread_cap \<leftarrow> get_cap tcb_cap_slot;
+     when (thread_cap = TcbCap target_tcb)
+          (insert_cap_child (fst pcap) (snd pcap) (target_tcb, target_slot) \<sqinter>
+           insert_cap_sibling (fst pcap) (snd pcap) (target_tcb,target_slot))
+   od)"
 
 (* Update a thread's CSpace root. *)
-definition
-  tcb_update_cspace_root :: "cdl_object_id \<Rightarrow> cdl_cap_ref \<Rightarrow> cdl_cap \<times> cdl_cap_ref \<Rightarrow> unit preempt_monad"
-where
-  "tcb_update_cspace_root target_tcb tcb_cap_ref croot \<equiv>
-  doE
+definition tcb_update_cspace_root ::
+  "cdl_object_id \<Rightarrow> cdl_cap_ref \<Rightarrow> cdl_cap \<times> cdl_cap_ref \<Rightarrow> unit preempt_monad"
+  where
+  "tcb_update_cspace_root target_tcb tcb_cap_ref croot \<equiv> doE
      tcb_empty_thread_slot target_tcb tcb_cspace_slot;
      src_cap \<leftarrow> liftE $ get_cap (snd croot);
-     whenE (is_cnode_cap src_cap \<and> (cap_object src_cap = cap_object (fst croot)))
-       $ tcb_update_thread_slot target_tcb tcb_cap_ref tcb_cspace_slot croot
-  odE"
+     whenE (is_cnode_cap src_cap \<and> cap_object src_cap = cap_object (fst croot)) $
+       tcb_update_thread_slot target_tcb tcb_cap_ref tcb_cspace_slot croot
+   odE"
 
 (* Update a thread's VSpace root. *)
-definition
-  tcb_update_vspace_root :: "cdl_object_id \<Rightarrow> cdl_cap_ref \<Rightarrow> (cdl_cap \<times> cdl_cap_ref) \<Rightarrow> unit preempt_monad"
-where
-  "tcb_update_vspace_root target_tcb tcb_cap_ref vroot \<equiv>
-  doE
+definition tcb_update_vspace_root ::
+  "cdl_object_id \<Rightarrow> cdl_cap_ref \<Rightarrow> (cdl_cap \<times> cdl_cap_ref) \<Rightarrow> unit preempt_monad"
+  where
+  "tcb_update_vspace_root target_tcb tcb_cap_ref vroot \<equiv> doE
      tcb_empty_thread_slot target_tcb tcb_vspace_slot;
      src_cap \<leftarrow> liftE $ get_cap (snd vroot);
-     whenE (cdl_same_arch_obj_as (fst vroot) src_cap)
-       $ tcb_update_thread_slot target_tcb tcb_cap_ref tcb_vspace_slot vroot
-  odE"
-
-
+     whenE (cdl_same_arch_obj_as (fst vroot) src_cap) $
+       tcb_update_thread_slot target_tcb tcb_cap_ref tcb_vspace_slot vroot
+   odE"
 
 (* Modify the TCB's intent to indicate an error during decode. *)
-definition
-  mark_tcb_intent_error :: "cdl_object_id \<Rightarrow> bool \<Rightarrow> unit k_monad"
-where
+definition mark_tcb_intent_error :: "cdl_object_id \<Rightarrow> bool \<Rightarrow> unit k_monad" where
   "mark_tcb_intent_error target_tcb has_error \<equiv>
-      update_thread target_tcb (\<lambda>t. (t\<lparr>cdl_tcb_intent := (cdl_tcb_intent t)\<lparr>cdl_intent_error := has_error\<rparr>\<rparr>))"
+     update_thread target_tcb
+       (\<lambda>t. (t\<lparr>cdl_tcb_intent := (cdl_tcb_intent t)\<lparr>cdl_intent_error := has_error\<rparr>\<rparr>))"
 
 (* Update a thread's IPC buffer. *)
+definition tcb_update_ipc_buffer ::
+  "cdl_object_id \<Rightarrow> cdl_cap_ref \<Rightarrow> (cdl_cap \<times> cdl_cap_ref) \<Rightarrow> unit preempt_monad"
+  where
+  "tcb_update_ipc_buffer target_tcb tcb_cap_ref ipc_buffer \<equiv> doE
+     tcb_empty_thread_slot target_tcb tcb_ipcbuffer_slot;
+     liftE $ corrupt_tcb_intent target_tcb;
+     src_cap \<leftarrow> liftE $ get_cap (snd ipc_buffer);
+     whenE (cdl_same_arch_obj_as (fst ipc_buffer) src_cap) $
+       tcb_update_thread_slot target_tcb tcb_cap_ref tcb_ipcbuffer_slot ipc_buffer
+   odE"
 
-definition
-  tcb_update_ipc_buffer :: "cdl_object_id \<Rightarrow> cdl_cap_ref \<Rightarrow> (cdl_cap \<times> cdl_cap_ref) \<Rightarrow> unit preempt_monad"
-where
-  "tcb_update_ipc_buffer target_tcb tcb_cap_ref ipc_buffer \<equiv>
-     doE
-       tcb_empty_thread_slot target_tcb tcb_ipcbuffer_slot;
-       liftE $ corrupt_tcb_intent target_tcb;
-       src_cap \<leftarrow> liftE $ get_cap (snd ipc_buffer);
-       whenE (cdl_same_arch_obj_as (fst ipc_buffer) src_cap)
-         $ tcb_update_thread_slot target_tcb tcb_cap_ref tcb_ipcbuffer_slot ipc_buffer
-     odE
-"
+(* Resume a thread, aborting any pending operation, and revoking any incoming reply caps. *)
+definition restart :: "cdl_object_id \<Rightarrow> unit k_monad" where
+  "restart target_tcb \<equiv> do
+     cap \<leftarrow> get_cap (target_tcb, tcb_pending_op_slot);
+     when (cap \<noteq> RestartCap \<and> cap \<noteq> RunningCap) $ do
+       cancel_ipc target_tcb;
+       set_cap (target_tcb, tcb_replycap_slot) (MasterReplyCap target_tcb);
+       set_cap (target_tcb, tcb_pending_op_slot) (RestartCap)
+     od
+   od"
 
-(* Resume a thread, aborting any pending operation, and revoking
- * any incoming reply caps. *)
-definition
-  restart :: "cdl_object_id \<Rightarrow> unit k_monad"
-where
-  "restart target_tcb \<equiv>
-  do
-     cap \<leftarrow> KHeap_D.get_cap (target_tcb,tcb_pending_op_slot);
-     when (cap \<noteq> RestartCap \<and> cap\<noteq> RunningCap)
-     (do
-       CSpace_D.cancel_ipc target_tcb;
-       KHeap_D.set_cap (target_tcb,tcb_replycap_slot) (cdl_cap.MasterReplyCap target_tcb);
-       KHeap_D.set_cap (target_tcb,tcb_pending_op_slot) (cdl_cap.RestartCap)
-      od)
-  od"
+(* Suspend a thread, aborting any pending operation, and revoking any incoming reply caps. *)
+definition suspend :: "cdl_object_id \<Rightarrow> unit k_monad" where
+  "suspend target_tcb \<equiv> do
+     cancel_ipc target_tcb;
+     set_cap (target_tcb, tcb_pending_op_slot) NullCap
+   od"
 
-(* Suspend a thread, aborting any pending operation, and revoking
- * any incoming reply caps. *)
-definition
-  suspend :: "cdl_object_id \<Rightarrow> unit k_monad"
-where
-  "suspend target_tcb \<equiv> CSpace_D.cancel_ipc target_tcb >>= K (KHeap_D.set_cap (target_tcb,tcb_pending_op_slot) cdl_cap.NullCap)"
+definition bind_notification :: "cdl_object_id \<Rightarrow> cdl_object_id \<Rightarrow> unit k_monad" where
+  "bind_notification tcb_id ntfn_id \<equiv>
+     set_cap (tcb_id, tcb_boundntfn_slot) (BoundNotificationCap ntfn_id)"
 
-definition
-  bind_notification :: "cdl_object_id \<Rightarrow> cdl_object_id \<Rightarrow> unit k_monad"
-where
-  "bind_notification tcb_id ntfn_id \<equiv> set_cap (tcb_id, tcb_boundntfn_slot) (BoundNotificationCap ntfn_id)"
+definition invoke_tcb :: "cdl_tcb_invocation \<Rightarrow> unit preempt_monad" where
+  "invoke_tcb params \<equiv>
+     case params of
+       \<comment> \<open>Modify a thread's registers.\<close>
+       WriteRegisters target_tcb resume _ _ \<Rightarrow>
+         liftE $ do
+           corrupt_tcb_intent target_tcb;
+           when resume $ restart target_tcb
+         od
 
-definition
-  invoke_tcb :: "cdl_tcb_invocation \<Rightarrow> unit preempt_monad"
-where
-  "invoke_tcb params \<equiv> case params of
-    \<comment> \<open>Modify a thread's registers.\<close>
-      WriteRegisters target_tcb resume _ _ \<Rightarrow>
-        liftE $
-        do
-          corrupt_tcb_intent target_tcb;
-          when resume $ restart target_tcb
-        od
+       \<comment> \<open>Read a thread's registers.\<close>
+     | ReadRegisters src_tcb _ _ _ \<Rightarrow>
+         liftE $ suspend src_tcb \<sqinter> return ()
 
-    \<comment> \<open>Read a thread's registers.\<close>
-    | ReadRegisters src_tcb _ _ _ \<Rightarrow>
-        liftE $ suspend src_tcb \<sqinter> return ()
+     \<comment> \<open>Copy registers from one thread to another\<close>
+     | CopyRegisters target_tcb source_tcb _ _ _ _ _ \<Rightarrow>
+         liftE $ do
+           suspend source_tcb \<sqinter> return ();
+           restart target_tcb \<sqinter> return ();
+           corrupt_tcb_intent target_tcb
+         od
 
-    \<comment> \<open>Copy registers from one thread to another\<close>
-    | CopyRegisters target_tcb source_tcb _ _ _ _ _ \<Rightarrow>
-        liftE $
-        do
-          suspend source_tcb \<sqinter> return ();
-          restart target_tcb \<sqinter> return ();
-          corrupt_tcb_intent target_tcb
-       od
+     \<comment> \<open>Suspend this thread.\<close>
+     | Suspend target_tcb \<Rightarrow>
+         liftE $ suspend target_tcb \<sqinter> return ()
 
-    \<comment> \<open>Suspend this thread.\<close>
-    | Suspend target_tcb \<Rightarrow>
-        liftE $ suspend target_tcb \<sqinter> return ()
+     \<comment> \<open>Resume this thread.\<close>
+     | Resume target_tcb \<Rightarrow>
+         liftE $ restart target_tcb
 
-    \<comment> \<open>Resume this thread.\<close>
-    | Resume target_tcb \<Rightarrow>
-        liftE $ restart target_tcb
+     \<comment> \<open>Update a thread's options.\<close>
+     | ThreadControl target_tcb tcb_cap_slot faultep croot vroot ipc_buffer \<Rightarrow> doE
+         case faultep of
+            Some x \<Rightarrow> liftE $ update_thread target_tcb (\<lambda>tcb. tcb\<lparr>cdl_tcb_fault_endpoint := x\<rparr>)
+         | None \<Rightarrow> returnOk ();
 
-    \<comment> \<open>Update a thread's options.\<close>
-    | ThreadControl target_tcb tcb_cap_slot faultep croot vroot ipc_buffer \<Rightarrow>
-        doE
-          case faultep of
-              Some x \<Rightarrow> liftE $ update_thread target_tcb (\<lambda>tcb. tcb\<lparr>cdl_tcb_fault_endpoint := x\<rparr>)
-            | None \<Rightarrow> returnOk ();
+         \<comment> \<open>Possibly update CSpace\<close>
+         case croot of
+           Some x \<Rightarrow> tcb_update_cspace_root target_tcb tcb_cap_slot x
+         | None \<Rightarrow> returnOk ();
 
-          \<comment> \<open>Possibly update CSpace\<close>
-          case croot of
-              Some x \<Rightarrow> tcb_update_cspace_root target_tcb tcb_cap_slot x
-            | None \<Rightarrow> returnOk ();
+         \<comment> \<open>Possibly update VSpace\<close>
+         case vroot of
+           Some x \<Rightarrow> tcb_update_vspace_root target_tcb tcb_cap_slot x
+         | None \<Rightarrow> returnOk ();
 
-          \<comment> \<open>Possibly update VSpace\<close>
-          case vroot of
-              Some x \<Rightarrow> tcb_update_vspace_root target_tcb tcb_cap_slot x
-            | None \<Rightarrow> returnOk ();
-
-          \<comment> \<open>Possibly update Ipc Buffer\<close>
-          case ipc_buffer of
-              Some x \<Rightarrow> tcb_update_ipc_buffer target_tcb tcb_cap_slot x
-            | None \<Rightarrow> (returnOk () \<sqinter> (doE tcb_empty_thread_slot target_tcb tcb_ipcbuffer_slot;
-                 liftE $ corrupt_tcb_intent target_tcb odE))
-        odE
-    | NotificationControl tcb ntfn \<Rightarrow>
-          liftE $ (case ntfn of
-             Some ntfn_id \<Rightarrow> bind_notification tcb ntfn_id
-           | None \<Rightarrow> unbind_notification tcb)
-    | SetTLSBase tcb \<Rightarrow> liftE $ corrupt_tcb_intent tcb
-    | SetFlags tcb set_flags clear_flags \<Rightarrow> liftE $ corrupt_tcb_intent tcb"
+         \<comment> \<open>Possibly update Ipc Buffer\<close>
+         case ipc_buffer of
+           Some x \<Rightarrow> tcb_update_ipc_buffer target_tcb tcb_cap_slot x
+         | None \<Rightarrow> returnOk () \<sqinter>
+                   doE
+                     tcb_empty_thread_slot target_tcb tcb_ipcbuffer_slot;
+                     liftE $ corrupt_tcb_intent target_tcb
+                   odE
+       odE
+     | NotificationControl tcb ntfn \<Rightarrow>
+         liftE (case ntfn of
+                  Some ntfn_id \<Rightarrow> bind_notification tcb ntfn_id
+                | None \<Rightarrow> unbind_notification tcb)
+     | SetTLSBase tcb \<Rightarrow> liftE $ corrupt_tcb_intent tcb
+     | SetFlags tcb set_flags clear_flags \<Rightarrow> liftE $ corrupt_tcb_intent tcb"
 
 
 (* Domain invocations *)
-
-definition
-  decode_domain_invocation :: "(cdl_cap \<times> cdl_cap_ref) list \<Rightarrow> cdl_domain_intent \<Rightarrow> cdl_domain_invocation except_monad"
-where
+definition decode_domain_invocation ::
+  "(cdl_cap \<times> cdl_cap_ref) list \<Rightarrow> cdl_domain_intent \<Rightarrow> cdl_domain_invocation except_monad"
+  where
   "decode_domain_invocation caps intent \<equiv> case intent of
      DomainSetIntent d \<Rightarrow>
        returnOk (InvokeSetDomain (cap_object (fst (hd caps))) d) \<sqinter> throw
@@ -311,25 +294,17 @@ where
    | DomainScheduleConfigureIntent idx domain duration \<Rightarrow>
        returnOk (InvokeDomainScheduleConfigure idx domain duration) \<sqinter> throw"
 
-definition
-  set_domain :: "cdl_object_id \<Rightarrow> domain \<Rightarrow> unit k_monad"
-where
+definition set_domain :: "cdl_object_id \<Rightarrow> domain \<Rightarrow> unit k_monad" where
   "set_domain tcb d \<equiv> update_thread tcb (\<lambda>t. (t\<lparr>cdl_tcb_domain := d \<rparr>))"
 
-definition
-  dom_schedule_set_start :: "nat \<Rightarrow> unit k_monad"
-where
+definition dom_schedule_set_start :: "nat \<Rightarrow> unit k_monad" where
   "dom_schedule_set_start start \<equiv> modify (\<lambda>s. s\<lparr> cdl_dom_start := start \<rparr>)"
 
-definition
-  dom_schedule_configure :: "nat \<Rightarrow> word8 \<Rightarrow> domain_duration \<Rightarrow> unit k_monad"
-where
+definition dom_schedule_configure :: "nat \<Rightarrow> word8 \<Rightarrow> domain_duration \<Rightarrow> unit k_monad" where
   "dom_schedule_configure idx domain duration \<equiv>
      modify (\<lambda>s. s\<lparr> cdl_dom_schedule := (cdl_dom_schedule s)[idx := (domain, duration)] \<rparr>)"
 
-definition
-  invoke_domain :: "cdl_domain_invocation \<Rightarrow> unit k_monad"
-where
+definition invoke_domain :: "cdl_domain_invocation \<Rightarrow> unit k_monad" where
   "invoke_domain params \<equiv> case params of
      InvokeSetDomain tcb d \<Rightarrow> set_domain tcb d
    | InvokeDomainScheduleSetStart start \<Rightarrow> dom_schedule_set_start start
