spec/capDL/Untyped_D.thy
@@ -4,56 +4,54 @@
  * SPDX-License-Identifier: GPL-2.0-only
  *)
 
-(*
- * Operations on untyped memory objects.
- *)
+(* Operations on untyped memory objects. *)
 
 theory Untyped_D
-imports Invocations_D CSpace_D Structures_D
+  imports
+    Invocations_D
+    CSpace_D
+    Structures_D
 begin
 
-definition
-  decode_untyped_invocation :: "cdl_cap \<Rightarrow> cdl_cap_ref \<Rightarrow> (cdl_cap \<times> cdl_cap_ref) list \<Rightarrow>
-      cdl_untyped_intent \<Rightarrow> cdl_untyped_invocation except_monad"
-where
-  "decode_untyped_invocation untyped_cap untyped_ref caps intent \<equiv> case intent of
-     UntypedRetypeIntent type size_bits node_index node_depth node_offset node_window \<Rightarrow>
-       doE
+definition decode_untyped_invocation ::
+  "cdl_cap \<Rightarrow> cdl_cap_ref \<Rightarrow> (cdl_cap \<times> cdl_cap_ref) list \<Rightarrow> cdl_untyped_intent \<Rightarrow>
+   cdl_untyped_invocation except_monad"
+  where
+  "decode_untyped_invocation untyped_cap untyped_ref caps intent \<equiv>
+     case intent of
+       UntypedRetypeIntent type size_bits node_index node_depth node_offset node_window \<Rightarrow> doE
          (root_cap, root_slot) \<leftarrow> throw_on_none $ get_index caps 0;
 
          \<comment> \<open>Lookup the destination slots.\<close>
-         target_node \<leftarrow> if node_depth = 0 then
-             returnOk root_cap
-           else
-             doE
-               target_slot \<leftarrow> lookup_slot_for_cnode_op root_cap node_index (unat node_depth);
-               liftE $ get_cap target_slot
-             odE;
+         target_node \<leftarrow>
+           if node_depth = 0
+           then returnOk root_cap
+           else doE
+             target_slot \<leftarrow> lookup_slot_for_cnode_op root_cap node_index (unat node_depth);
+             liftE $ get_cap target_slot
+           odE;
 
          \<comment> \<open>Ensure it is a CNode cap.\<close>
          unlessE (is_cnode_cap target_node) throw;
 
          \<comment> \<open>Find our target slots.\<close>
          slots \<leftarrow> returnOk $ map (\<lambda>n. (cap_object target_node, n))
-               [unat node_offset ..< unat node_offset + unat node_window];
+                                 [unat node_offset ..< unat node_offset + unat node_window];
          mapME_x ensure_empty slots;
 
-         \<comment> \<open>Work out what names are available. If we haven't haven't already been typed into something we can reuse our names.\<close>
+         \<comment> \<open>Work out what names are available. If we haven't haven't already been typed into
+             something we can reuse our names.\<close>
          s \<leftarrow> liftE $ get;
          has_kids \<leftarrow> returnOk $ has_children untyped_ref s;
 
          returnOk $ Retype untyped_ref type (unat size_bits) slots has_kids (unat node_window)
-       odE \<sqinter> throw"
+       odE
+       \<sqinter> throw"
 
 (* Zero out a set of addresses. *)
-definition
-  detype :: "cdl_object_id set \<Rightarrow> cdl_state \<Rightarrow> cdl_state"
-where
+definition detype :: "cdl_object_id set \<Rightarrow> cdl_state \<Rightarrow> cdl_state" where
   "detype detype_set s \<equiv>
-     (s\<lparr> cdl_objects :=
-         (\<lambda>x. if x \<in> detype_set then
-           Some Untyped
-         else cdl_objects s x)\<rparr>)"
+     s\<lparr>cdl_objects := \<lambda>x. if x \<in> detype_set then Some Untyped else cdl_objects s x\<rparr>"
 
 (* Return a list of num_objects sets for requested the request number of objects;
    if the object type is not UntypedType, the sets contain a singleton ptr for the
@@ -67,35 +65,30 @@ definition generate_range ::
              [0 ..< num_objects]"
 
 definition create_objects :: "(cdl_object_id set) list \<Rightarrow> cdl_object option \<Rightarrow> unit k_monad"
-where
+  where
   "create_objects target_object_ids object \<equiv>
-    (modify (\<lambda>s. s\<lparr>cdl_objects := (\<lambda>x.
-     if {x} \<in> set target_object_ids then
-      object
-     else
-      cdl_objects s x)\<rparr>))"
+     modify (\<lambda>s. s\<lparr>cdl_objects := (\<lambda>x. if {x} \<in> set target_object_ids
+                                       then object
+                                       else cdl_objects s x)\<rparr>)"
 
 
 (* Insert a cap for a new object in the given location. *)
-definition
-  create_cap :: "cdl_object_type \<Rightarrow> nat \<Rightarrow> cdl_cap_ref \<Rightarrow> bool \<Rightarrow> (cdl_cap_ref \<times> cdl_object_id set) \<Rightarrow> unit k_monad"
-where
-  "create_cap new_type sz parent_slot dev \<equiv> \<lambda>(dest_slot, obj_refs).
-  do
-    old_cap \<leftarrow> get_cap dest_slot;
-    assert (old_cap = NullCap);
-    set_cap dest_slot (default_cap new_type obj_refs sz dev);
-    set_parent dest_slot parent_slot
-  od"
+definition create_cap ::
+  "cdl_object_type \<Rightarrow> nat \<Rightarrow> cdl_cap_ref \<Rightarrow> bool \<Rightarrow> (cdl_cap_ref \<times> cdl_object_id set) \<Rightarrow> unit k_monad"
+  where
+  "create_cap new_type sz parent_slot dev \<equiv> \<lambda>(dest_slot, obj_refs). do
+     old_cap \<leftarrow> get_cap dest_slot;
+     assert (old_cap = NullCap);
+     set_cap dest_slot (default_cap new_type obj_refs sz dev);
+     set_parent dest_slot parent_slot
+   od"
 
 (* This returns the set of unused ptrs while explicitly checking for overflow *)
 definition update_range :: "cdl_object_id set \<Rightarrow> cdl_object_id \<Rightarrow> nat \<Rightarrow> cdl_object_id set" where
   "update_range old_range ptr idx \<equiv>
      if idx = 0
      then old_range
-     else if (ptr \<le> ptr + of_nat idx)
-       then old_range - {..<ptr + of_nat idx}
-       else {}"
+     else if ptr \<le> ptr + of_nat idx then old_range - {..<ptr + of_nat idx} else {}"
 
 definition update_available_range ::
   "cdl_object_id \<Rightarrow> nat \<Rightarrow> cdl_cap_ref \<Rightarrow> cdl_cap \<Rightarrow> unit k_monad"
@@ -108,44 +101,33 @@ definition update_available_range ::
 definition retype_region ::
   "nat \<Rightarrow> cdl_object_type \<Rightarrow> (cdl_object_id set list) \<Rightarrow> ((cdl_object_id set) list) k_monad"
   where
-  "retype_region target_bits target_type target_object_ids \<equiv>
-    do
-      \<comment> \<open>Get a list of target locations. We are happy with any unused name
-         within the target range.\<close>
+  "retype_region target_bits target_type target_object_ids \<equiv> do
+     if target_type \<noteq> UntypedType
+     then do
+       current_domain \<leftarrow> gets cdl_current_domain;
+       create_objects target_object_ids (default_object target_type target_bits current_domain)
+     od
+     else return ();
 
-      if (target_type \<noteq> UntypedType) then
-       do
-         current_domain \<leftarrow> gets cdl_current_domain;
-         create_objects target_object_ids (default_object target_type target_bits current_domain)
-       od
-      else return ();
+     return target_object_ids
+   od"
 
-      \<comment> \<open>Get a list of target locations. We are happy with any unused name
-         within the target range.\<close>
-      return target_object_ids
-    od"
+primrec (nonexhaustive) untyped_is_device :: "cdl_cap \<Rightarrow> bool" where
+  "untyped_is_device (UntypedCap d _ _) = d"
 
-primrec (nonexhaustive)
-  untyped_is_device :: "cdl_cap \<Rightarrow> bool"
-where
-    "untyped_is_device (UntypedCap d _ _) = d"
-
-definition
-  reset_untyped_cap :: "cdl_cap_ref \<Rightarrow> unit preempt_monad"
-where
+definition reset_untyped_cap :: "cdl_cap_ref \<Rightarrow> unit preempt_monad" where
   "reset_untyped_cap cref \<equiv> doE
-    cap \<leftarrow> liftE $ get_cap cref;
-    whenE (available_range cap \<noteq> cap_objects cap) $ doE
-      liftE $ modify (detype (cap_objects cap));
-      new_rans \<leftarrow> liftE $ select {xs. (\<forall>S \<in> set xs.
-              S \<subseteq> cap_objects cap \<and> available_range cap \<subset> S)
-          \<and> xs \<noteq> [] \<and> List.last xs = cap_objects cap};
-      mapME_x (\<lambda>r. doE
-        liftE $ set_cap cref $ set_available_range cap r;
-        returnOk () \<sqinter> throw
-      odE) new_rans
-    odE
-  odE"
+     cap \<leftarrow> liftE $ get_cap cref;
+     whenE (available_range cap \<noteq> cap_objects cap) $ doE
+       liftE $ modify (detype (cap_objects cap));
+       new_rans \<leftarrow> liftE $ select {xs. (\<forall>S \<in> set xs. S \<subseteq> cap_objects cap \<and> available_range cap \<subset> S)
+                                       \<and> xs \<noteq> [] \<and> List.last xs = cap_objects cap};
+       mapME_x (\<lambda>r. doE
+         liftE $ set_cap cref $ set_available_range cap r;
+         returnOk () \<sqinter> throw
+       odE) new_rans
+     odE
+   odE"
 
 definition pte_bits :: nat where
   "pte_bits \<equiv> if word_bits = 32 then 2 else 3"
@@ -174,42 +156,43 @@ definition keep_if :: "('a \<Rightarrow> bool) \<Rightarrow> 'a \<Rightarrow> 'a
 abbreviation min_of_range :: "'a set \<Rightarrow> 'a set \<Rightarrow> 'a::linorder" where
   "min_of_range r1 r2 \<equiv> Min (keep_if ((\<noteq>) {}) r1 r2)"
 
-definition
-  invoke_untyped :: "cdl_untyped_invocation \<Rightarrow> unit preempt_monad"
-where
-  "invoke_untyped params \<equiv> case params of
-     Retype untyped_ref new_type type_size target_slots has_kids num_objects \<Rightarrow>
-   doE
-     unlessE has_kids $ reset_untyped_cap untyped_ref;
-       liftE $ do
-         untyped_cap  \<leftarrow> get_cap untyped_ref;
+definition invoke_untyped :: "cdl_untyped_invocation \<Rightarrow> unit preempt_monad" where
+  "invoke_untyped params \<equiv>
+     case params of
+       Retype untyped_ref new_type type_size target_slots has_kids num_objects \<Rightarrow> doE
+         unlessE has_kids $ reset_untyped_cap untyped_ref;
+         liftE $ do
+           untyped_cap \<leftarrow> get_cap untyped_ref;
 
-         base_ptr     \<leftarrow> return $ Min (untyped_cap_range untyped_cap);
+           base_ptr \<leftarrow> return $ Min (untyped_cap_range untyped_cap);
 
-         \<comment> \<open>If we have overflow, then the available range will be empty,
-            but the index is considered to have wrapped back around to zero.\<close>
-         next_ptr     \<leftarrow> return $ min_of_range (available_range untyped_cap)
-                                               (untyped_cap_range untyped_cap);
+           \<comment> \<open>If we have overflow, then the available range will be empty,
+              but the index is considered to have wrapped back around to zero.\<close>
+           next_ptr \<leftarrow> return $ min_of_range (available_range untyped_cap)
+                                             (untyped_cap_range untyped_cap);
 
-         \<comment> \<open> Check if the ptr needs aligning \<close>
-         aligned_ptr  \<leftarrow> return $ if has_kids then alignUp next_ptr (obj_bits_cdl new_type type_size) else next_ptr;
+           \<comment> \<open> Check if the ptr needs aligning \<close>
+           aligned_ptr \<leftarrow> return $ if has_kids
+                                   then alignUp next_ptr (obj_bits_cdl new_type type_size)
+                                   else next_ptr;
 
-         new_obj_refs \<leftarrow> return $ generate_range (aligned_ptr) new_type (obj_bits_cdl new_type type_size) num_objects;
-         new_idx      \<leftarrow> return $ aligned_ptr + (of_nat num_objects << (obj_bits_cdl new_type type_size)) - base_ptr;
+           new_obj_refs \<leftarrow> return $ generate_range (aligned_ptr) new_type
+                                                   (obj_bits_cdl new_type type_size) num_objects;
+           new_idx      \<leftarrow> return $ aligned_ptr
+                                    + (of_nat num_objects << (obj_bits_cdl new_type type_size))
+                                    - base_ptr;
 
-         update_available_range base_ptr (unat (new_idx)) untyped_ref untyped_cap;
+           update_available_range base_ptr (unat (new_idx)) untyped_ref untyped_cap;
 
-         \<comment> \<open>Construct new objects within the covered range.\<close>
-         retype_region type_size new_type new_obj_refs;
+           \<comment> \<open>Construct new objects within the covered range.\<close>
+           retype_region type_size new_type new_obj_refs;
 
-         \<comment> \<open>Construct caps for the new objects.\<close>
-         mapM_x (create_cap new_type type_size untyped_ref (untyped_is_device untyped_cap)) (zip target_slots new_obj_refs);
+           \<comment> \<open>Construct caps for the new objects.\<close>
+           mapM_x (create_cap new_type type_size untyped_ref (untyped_is_device untyped_cap))
+                  (zip target_slots new_obj_refs);
 
-         \<comment> \<open>Ideally, we should return back to the user how many
-            objects were created.\<close>
-
-         return ()
-       od
-    odE"
+           return ()
+         od
+       odE"
 
 end
